@prefix : <http://www.semanticweb.org/alecsculley/ontologies/2023/6/crimeontology#> .
@prefix owl: <http://www.w3.org/2002/07/owl#> .
@prefix rdf: <http://www.w3.org/1999/02/22-rdf-syntax-ns#> .
@prefix xml: <http://www.w3.org/XML/1998/namespace> .
@prefix xsd: <http://www.w3.org/2001/XMLSchema#> .
@prefix rdfs: <http://www.w3.org/2000/01/rdf-schema#> .
@base <http://www.semanticweb.org/alecsculley/ontologies/2023/6/crimeontology> .

<http://www.semanticweb.org/alecsculley/ontologies/2023/6/crimeontology> rdf:type owl:Ontology ;
                                                                          owl:imports <http://purl.obolibrary.org/obo/bfo/2020/notime/bfo.owl> .

#################################################################
#    Annotation properties
#################################################################

###  http://www.ontologyrepository.com/CommonCoreOntologies/definition_source
<http://www.ontologyrepository.com/CommonCoreOntologies/definition_source> rdf:type owl:AnnotationProperty .


#################################################################
#    Classes
#################################################################

###  http://www.semanticweb.org/alecsculley/ontologies/2023/6/crimeontology#OWLClass_01941403_ff94_48f1_9377_c187032b4f53
:OWLClass_01941403_ff94_48f1_9377_c187032b4f53 rdf:type owl:Class ;
                                               rdfs:subClassOf :OWLClass_09a1351d_0eae_43fd_8841_989b08e40a54 ;
                                               rdfs:isDefinedBy "https://bjs.ojp.gov/sites/g/files/xyckuh236/files/sarble/data_common/nibrs-user-manual-2021-1041521.pdf" ;
                                               rdfs:label "Drug/Narcotic Offense"@en ;
                                               <http://www.w3.org/2004/02/skos/core#definition> "The violation of laws prohibiting the production, distribution, and/or use of certain controlled substances and the equipment or devices utilized in their preparation and/or use." .


###  http://www.semanticweb.org/alecsculley/ontologies/2023/6/crimeontology#OWLClass_01a675dc_525d_402b_a75b_84002d5715ff
:OWLClass_01a675dc_525d_402b_a75b_84002d5715ff rdf:type owl:Class ;
                                               rdfs:subClassOf :OWLClass_88536041_a2e5_48a7_8cd1_a21b8217d6e6 ;
                                               rdfs:isDefinedBy "https://bjs.ojp.gov/sites/g/files/xyckuh236/files/sarble/data_common/nibrs-user-manual-2021-1041521.pdf" ;
                                               rdfs:label "Harboring Escapee/Concealing from Arrest"@en ;
                                               <http://www.w3.org/2004/02/skos/core#definition> "To harbor or conceal any person for whose arrest, a warrant or process has been issued, so as to prevent the fugitive's discovery and arrest, after having notice or knowledge that a warrant or process has been issued for the fugitive's apprehension." .


###  http://www.semanticweb.org/alecsculley/ontologies/2023/6/crimeontology#OWLClass_031abc3c_4c7c_4f2d_89d4_a17258417b93
:OWLClass_031abc3c_4c7c_4f2d_89d4_a17258417b93 rdf:type owl:Class ;
                                               rdfs:subClassOf :OWLClass_01941403_ff94_48f1_9377_c187032b4f53 ;
                                               rdfs:isDefinedBy "https://bjs.ojp.gov/sites/g/files/xyckuh236/files/sarble/data_common/nibrs-user-manual-2021-1041521.pdf" ;
                                               rdfs:label "Drug/Narcotic Violation"@en ;
                                               <http://www.w3.org/2004/02/skos/core#definition> "The unlawful cultivation, manufacture, distribution, sale, purchase, use, possession, transportation, or importation of any controlled substance." .


###  http://www.semanticweb.org/alecsculley/ontologies/2023/6/crimeontology#OWLClass_04c8931b_7445_4b70_a44a_34563a22ef3b
:OWLClass_04c8931b_7445_4b70_a44a_34563a22ef3b rdf:type owl:Class ;
                                               rdfs:subClassOf :OWLClass_d6aabe44_4c76_4912_b4ee_6ff6278fa214 ;
                                               rdfs:isDefinedBy "https://bjs.ojp.gov/sites/g/files/xyckuh236/files/sarble/data_common/nibrs-user-manual-2021-1041521.pdf" ;
                                               rdfs:label "Identity Theft"@en ;
                                               <http://www.w3.org/2004/02/skos/core#definition> "Wrongfully obtaining and/or using another person’s personal data (e.g., name and date of birth, Social Security number, driver’s license number)." .


###  http://www.semanticweb.org/alecsculley/ontologies/2023/6/crimeontology#OWLClass_0625c00d_9805_4639_9090_746645edcfde
:OWLClass_0625c00d_9805_4639_9090_746645edcfde rdf:type owl:Class ;
                                               rdfs:subClassOf :OWLClass_6700c269_d438_4dcd_aa44_fda517de5744 ;
                                               rdfs:isDefinedBy "https://bjs.ojp.gov/sites/g/files/xyckuh236/files/sarble/data_common/nibrs-user-manual-2021-1041521.pdf" ;
                                               rdfs:label "Federal Liquor Offense"@en ;
                                               <http://www.w3.org/2004/02/skos/core#definition> "The unlawful production (using an unregistered still), transportation (without proper bill of lading), receipt, distribution, or smuggling of distilled spirits on which federal tax has not been paid. Acting as a distiller, a winery, or a wholesaler of distilled spirits, wine, or malt beverages without a federal permit." .


###  http://www.semanticweb.org/alecsculley/ontologies/2023/6/crimeontology#OWLClass_09a1351d_0eae_43fd_8841_989b08e40a54
:OWLClass_09a1351d_0eae_43fd_8841_989b08e40a54 rdf:type owl:Class ;
                                               rdfs:subClassOf :OWLClass_698d3768_6ed4_4042_88af_0f05dc222535 ;
                                               <http://www.ontologyrepository.com/CommonCoreOntologies/definition_source> "https://bjs.ojp.gov/sites/g/files/xyckuh236/files/sarble/data_common/nibrs-user-manual-2021-1041521.pdf" ;
                                               rdfs:label "Crime Against Society"@en ;
                                               <http://www.w3.org/2004/02/skos/core#definition> "A crime against society is a crime that society prohibits, but which is not a crime against persons or a crime against property." .


###  http://www.semanticweb.org/alecsculley/ontologies/2023/6/crimeontology#OWLClass_0bdcbb40_9669_4246_8b85_44f5315a9cfa
:OWLClass_0bdcbb40_9669_4246_8b85_44f5315a9cfa rdf:type owl:Class ;
                                               rdfs:subClassOf :OWLClass_a8a577c3_d157_42d4_bd84_b53f80c7044c ;
                                               rdfs:isDefinedBy "https://bjs.ojp.gov/sites/g/files/xyckuh236/files/sarble/data_common/nibrs-user-manual-2021-1041521.pdf" ;
                                               rdfs:label "Violation of National Firearms Act of 1934"@en ;
                                               <http://www.w3.org/2004/02/skos/core#definition> "To manufacture, import, sell, purchase, transfer, possess, or transport in interstate commerce, a firearm knowing it has the characteristics or features of a short barreled rifle or shotgun, machine gun, silencer, destructive device, or any other weapon as defined at 26 USC § 5845(a) in violation of the provisions of the National Firearms Act (generally non-tax paid, unregistered)." .


###  http://www.semanticweb.org/alecsculley/ontologies/2023/6/crimeontology#OWLClass_0be0fff2_6aac_44b7_af4e_d5708695a424
:OWLClass_0be0fff2_6aac_44b7_af4e_d5708695a424 rdf:type owl:Class ;
                                               rdfs:subClassOf :OWLClass_b3e5e274_46a8_4fe5_a1d2_f72c3fda9bf6 ;
                                               rdfs:isDefinedBy "https://bjs.ojp.gov/sites/g/files/xyckuh236/files/sarble/data_common/nibrs-user-manual-2021-1041521.pdf" ;
                                               rdfs:label "Gambling Equipment Violations"@en ;
                                               <http://www.w3.org/2004/02/skos/core#definition> "To unlawfully manufacture, sell, buy, possess, or transport equipment, devices, and/or goods used for gambling purposes." .


###  http://www.semanticweb.org/alecsculley/ontologies/2023/6/crimeontology#OWLClass_13060433_edbf_436f_97a7_6dc13a59693a
:OWLClass_13060433_edbf_436f_97a7_6dc13a59693a rdf:type owl:Class ;
                                               rdfs:subClassOf :OWLClass_ab1951b1_39ec_4ccc_af50_2a3e76f9b5ed ;
                                               owl:disjointWith :OWLClass_c587f60d_3028_477e_979d_40fee70db23c ;
                                               rdfs:isDefinedBy "https://bjs.ojp.gov/sites/g/files/xyckuh236/files/sarble/data_common/nibrs-user-manual-2021-1041521.pdf" ;
                                               rdfs:label "Murder and Nonnegligent Manslaughter"@en ;
                                               <http://www.w3.org/2004/02/skos/core#definition> "The willful (nonnegligent) killing of one human being by another." .


###  http://www.semanticweb.org/alecsculley/ontologies/2023/6/crimeontology#OWLClass_13a3be60_8fc3_45a2_bc5b_bc94f077bc6b
:OWLClass_13a3be60_8fc3_45a2_bc5b_bc94f077bc6b rdf:type owl:Class ;
                                               rdfs:subClassOf :OWLClass_93dc2b9e_a62b_4559_a478_fbffa91737ca ;
                                               rdfs:isDefinedBy "https://bjs.ojp.gov/sites/g/files/xyckuh236/files/sarble/data_common/nibrs-user-manual-2021-1041521.pdf" ;
                                               rdfs:label "Prostitution"@en ;
                                               <http://www.w3.org/2004/02/skos/core#definition> "To engage in commercial sex acts for anything of value." .


###  http://www.semanticweb.org/alecsculley/ontologies/2023/6/crimeontology#OWLClass_20216fa3_d400_4d05_b118_db40fb8f01e4
:OWLClass_20216fa3_d400_4d05_b118_db40fb8f01e4 rdf:type owl:Class ;
                                               rdfs:subClassOf :OWLClass_fabdd37c_04aa_4a14_bcc7_6a56bd65ffa4 ;
                                               rdfs:isDefinedBy "https://bjs.ojp.gov/sites/g/files/xyckuh236/files/sarble/data_common/nibrs-user-manual-2021-1041521.pdf" ;
                                               rdfs:label "False Citizenship"@en ;
                                               <http://www.w3.org/2004/02/skos/core#definition> "Falsely and willfully representing oneself to be a citizen of the United States." .


###  http://www.semanticweb.org/alecsculley/ontologies/2023/6/crimeontology#OWLClass_22f2f59c_a6b7_412e_8ec1_d61cbeca0ce8
:OWLClass_22f2f59c_a6b7_412e_8ec1_d61cbeca0ce8 rdf:type owl:Class ;
                                               rdfs:subClassOf :OWLClass_09a1351d_0eae_43fd_8841_989b08e40a54 ;
                                               rdfs:isDefinedBy "https://bjs.ojp.gov/sites/g/files/xyckuh236/files/sarble/data_common/nibrs-user-manual-2021-1041521.pdf" ;
                                               rdfs:label "Pornography/Obscene Material"@en ;
                                               <http://www.w3.org/2004/02/skos/core#definition> "The violation of laws or ordinances prohibiting the manufacture, publishing (publication), distributing (distribution), sale, purchase, or possession of sexually explicit material deemed legally obscene." .


###  http://www.semanticweb.org/alecsculley/ontologies/2023/6/crimeontology#OWLClass_275c50da_46a5_4715_a4e0_b0f5406e9820
:OWLClass_275c50da_46a5_4715_a4e0_b0f5406e9820 rdf:type owl:Class ;
                                               rdfs:subClassOf :OWLClass_bc6631dd_6969_4e1a_9221_1eb96781d318 ;
                                               rdfs:isDefinedBy "https://bjs.ojp.gov/sites/g/files/xyckuh236/files/sarble/data_common/nibrs-user-manual-2021-1041521.pdf" ;
                                               rdfs:label "Counterfeiting/Forgery"@en ;
                                               <http://www.w3.org/2004/02/skos/core#definition> "The altering, copying, or imitating of something, without authority or right, with the intent to deceive or defraud by passing the copy or thing altered or imitated as that which is original or genuine, or the selling, buying, or possession of an altered, copied, or imitated thing with the intent to deceive or defraud." .


###  http://www.semanticweb.org/alecsculley/ontologies/2023/6/crimeontology#OWLClass_2bf259d2_3ccc_4934_9b91_b6a3c2a73103
:OWLClass_2bf259d2_3ccc_4934_9b91_b6a3c2a73103 rdf:type owl:Class ;
                                               rdfs:subClassOf :OWLClass_ffc3cd08_93aa_46ec_819c_ba6a08344509 ;
                                               rdfs:isDefinedBy "https://bjs.ojp.gov/sites/g/files/xyckuh236/files/sarble/data_common/nibrs-user-manual-2021-1041521.pdf" ;
                                               rdfs:label "Pocket-picking"@en ;
                                               <http://www.w3.org/2004/02/skos/core#definition> "The theft of articles from another person’s physical possession by stealth where the victim is not immediately aware a theft occurred." .


###  http://www.semanticweb.org/alecsculley/ontologies/2023/6/crimeontology#OWLClass_3161b469_6ed6_4e04_bf54_33eb3df4b49b
:OWLClass_3161b469_6ed6_4e04_bf54_33eb3df4b49b rdf:type owl:Class ;
                                               rdfs:subClassOf :OWLClass_d6aabe44_4c76_4912_b4ee_6ff6278fa214 ;
                                               rdfs:isDefinedBy "https://bjs.ojp.gov/sites/g/files/xyckuh236/files/sarble/data_common/nibrs-user-manual-2021-1041521.pdf" ;
                                               rdfs:label "Wire Fraud"@en ;
                                               <http://www.w3.org/2004/02/skos/core#definition> "The use of an electric or electronic communications facility to intentionally transmit a false and/or deceptive message in furtherance of a fraudulent activity." .


###  http://www.semanticweb.org/alecsculley/ontologies/2023/6/crimeontology#OWLClass_32d0d6a3_956a_4433_8b09_8f7d0febe84c
:OWLClass_32d0d6a3_956a_4433_8b09_8f7d0febe84c rdf:type owl:Class ;
                                               rdfs:subClassOf :OWLClass_09a1351d_0eae_43fd_8841_989b08e40a54 ;
                                               rdfs:isDefinedBy "https://bjs.ojp.gov/sites/g/files/xyckuh236/files/sarble/data_common/nibrs-user-manual-2021-1041521.pdf" ;
                                               rdfs:label "Money Laundering"@en ;
                                               <http://www.w3.org/2004/02/skos/core#definition> "The process of transforming the profits of a crime into a legitimate asset." .


###  http://www.semanticweb.org/alecsculley/ontologies/2023/6/crimeontology#OWLClass_3305dd81_545d_4750_afc8_9221881757f8
:OWLClass_3305dd81_545d_4750_afc8_9221881757f8 rdf:type owl:Class ;
                                               rdfs:subClassOf :OWLClass_468582e8_7bed_4d62_816b_aca1037cec5c ;
                                               rdfs:isDefinedBy "https://bjs.ojp.gov/sites/g/files/xyckuh236/files/sarble/data_common/nibrs-user-manual-2021-1041521.pdf" ;
                                               rdfs:label "Incest"@en ;
                                               <http://www.w3.org/2004/02/skos/core#definition> "Nonforcible sexual intercourse between persons who are related to each other within the degrees wherein marriage is prohibited by law." .


###  http://www.semanticweb.org/alecsculley/ontologies/2023/6/crimeontology#OWLClass_3384efaa_3631_49f6_831f_108b94381362
:OWLClass_3384efaa_3631_49f6_831f_108b94381362 rdf:type owl:Class ;
                                               rdfs:subClassOf :OWLClass_bc6631dd_6969_4e1a_9221_1eb96781d318 ;
                                               rdfs:isDefinedBy "https://bjs.ojp.gov/sites/g/files/xyckuh236/files/sarble/data_common/nibrs-user-manual-2021-1041521.pdf" ;
                                               rdfs:label "Burglary/Breaking & Entering"@en ;
                                               <http://www.w3.org/2004/02/skos/core#definition> "The unlawful entry into a building or some other structure to commit a felony or a theft." .


###  http://www.semanticweb.org/alecsculley/ontologies/2023/6/crimeontology#OWLClass_342e0730_c70f_4afa_909f_1c443bae77ac
:OWLClass_342e0730_c70f_4afa_909f_1c443bae77ac rdf:type owl:Class ;
                                               rdfs:subClassOf :OWLClass_ffc3cd08_93aa_46ec_819c_ba6a08344509 ;
                                               rdfs:isDefinedBy "https://bjs.ojp.gov/sites/g/files/xyckuh236/files/sarble/data_common/nibrs-user-manual-2021-1041521.pdf" ;
                                               rdfs:label "Theft from Motor Vehicle"@en ;
                                               <http://www.w3.org/2004/02/skos/core#definition> "The unlawful taking of articles from a motor vehicle, locked or unlocked." .


###  http://www.semanticweb.org/alecsculley/ontologies/2023/6/crimeontology#OWLClass_398810e4_2b87_40a1_9ba3_2059acb81322
:OWLClass_398810e4_2b87_40a1_9ba3_2059acb81322 rdf:type owl:Class ;
                                               rdfs:subClassOf :OWLClass_bc6631dd_6969_4e1a_9221_1eb96781d318 ;
                                               rdfs:isDefinedBy "https://bjs.ojp.gov/sites/g/files/xyckuh236/files/sarble/data_common/nibrs-user-manual-2021-1041521.pdf" ;
                                               rdfs:label "Destruction/Damage/Vandalism of Property"@en ;
                                               <http://www.w3.org/2004/02/skos/core#definition> "To willfully or maliciously destroy, damage, deface, or otherwise injure any public or private property without the consent of the owner or the person having custody or control of it." .


###  http://www.semanticweb.org/alecsculley/ontologies/2023/6/crimeontology#OWLClass_3b713ed2_061e_496a_a6ca_bc924a3024eb
:OWLClass_3b713ed2_061e_496a_a6ca_bc924a3024eb rdf:type owl:Class ;
                                               rdfs:subClassOf :OWLClass_bc6631dd_6969_4e1a_9221_1eb96781d318 ;
                                               rdfs:isDefinedBy "https://bjs.ojp.gov/sites/g/files/xyckuh236/files/sarble/data_common/nibrs-user-manual-2021-1041521.pdf" ;
                                               rdfs:label "Extortion/Blackmail"@en ;
                                               <http://www.w3.org/2004/02/skos/core#definition> "To unlawfully obtain money, property, or any other thing of value, either tangible or intangible, through the use or threat of force, misuse of authority, threat of criminal prosecution, threat of destruction of reputation or social standing, or through other coercive means." .


###  http://www.semanticweb.org/alecsculley/ontologies/2023/6/crimeontology#OWLClass_3ee541f8_ad76_4a09_bfe3_80e17b381f91
:OWLClass_3ee541f8_ad76_4a09_bfe3_80e17b381f91 rdf:type owl:Class ;
                                               rdfs:subClassOf :OWLClass_bc6631dd_6969_4e1a_9221_1eb96781d318 ;
                                               rdfs:isDefinedBy "https://bjs.ojp.gov/sites/g/files/xyckuh236/files/sarble/data_common/nibrs-user-manual-2021-1041521.pdf" ;
                                               rdfs:label "Robbery"@en ;
                                               <http://www.w3.org/2004/02/skos/core#definition> "The taking of anything of value from the control, custody, or care of another person by force or threat of force and/or by putting the victim in fear of immediate harm." .


###  http://www.semanticweb.org/alecsculley/ontologies/2023/6/crimeontology#OWLClass_468582e8_7bed_4d62_816b_aca1037cec5c
:OWLClass_468582e8_7bed_4d62_816b_aca1037cec5c rdf:type owl:Class ;
                                               rdfs:subClassOf :OWLClass_4a556836_abaa_4c4b_93ae_bceaed442c48 ;
                                               rdfs:isDefinedBy "https://bjs.ojp.gov/sites/g/files/xyckuh236/files/sarble/data_common/nibrs-user-manual-2021-1041521.pdf" ;
                                               rdfs:label "Sex Offense"@en ;
                                               <http://www.w3.org/2004/02/skos/core#definition> """#1: Any sexual act directed against another person, without the consent of the victim, including instances where the victim is incapable of giving consent.

#2: Unlawful sexual intercourse.""" .


###  http://www.semanticweb.org/alecsculley/ontologies/2023/6/crimeontology#OWLClass_48331cbf_5784_4380_830b_a1aa865ed8ff
:OWLClass_48331cbf_5784_4380_830b_a1aa865ed8ff rdf:type owl:Class ;
                                               rdfs:subClassOf :OWLClass_09a1351d_0eae_43fd_8841_989b08e40a54 ;
                                               rdfs:isDefinedBy "https://bjs.ojp.gov/sites/g/files/xyckuh236/files/sarble/data_common/nibrs-user-manual-2021-1041521.pdf" ;
                                               rdfs:label "Espionage"@en ;
                                               <http://www.w3.org/2004/02/skos/core#definition> "The act of obtaining, delivering, transmitting, communicating, or receiving national security or national defense information with an intent, or reason to believe, that the information may be used to the injury of the United States or to the advantage of any foreign nation." .


###  http://www.semanticweb.org/alecsculley/ontologies/2023/6/crimeontology#OWLClass_4a556836_abaa_4c4b_93ae_bceaed442c48
:OWLClass_4a556836_abaa_4c4b_93ae_bceaed442c48 rdf:type owl:Class ;
                                               rdfs:subClassOf :OWLClass_698d3768_6ed4_4042_88af_0f05dc222535 ;
                                               <http://www.ontologyrepository.com/CommonCoreOntologies/definition_source> "https://bjs.ojp.gov/sites/g/files/xyckuh236/files/sarble/data_common/nibrs-user-manual-2021-1041521.pdf" ;
                                               rdfs:label "Crime Against a Person"@en ;
                                               <http://www.w3.org/2004/02/skos/core#definition> "A crime against a person is a crime whose victim is some individual." .


###  http://www.semanticweb.org/alecsculley/ontologies/2023/6/crimeontology#OWLClass_4b003f10_d59f_490b_91d9_6f2d122f6a5d
:OWLClass_4b003f10_d59f_490b_91d9_6f2d122f6a5d rdf:type owl:Class ;
                                               rdfs:subClassOf :OWLClass_7a3cf11d_bd4a_475d_a5a3_9cd5b5e015b4 ;
                                               rdfs:isDefinedBy "https://bjs.ojp.gov/sites/g/files/xyckuh236/files/sarble/data_common/nibrs-user-manual-2021-1041521.pdf" ;
                                               rdfs:label "Simple Assault"@en ;
                                               <http://www.w3.org/2004/02/skos/core#definition> "An unlawful physical attack by one person upon another where neither the offender displays a dangerous weapon, nor the victim suffers obvious severe or aggravated bodily injury involving apparent broken bones, loss of teeth, possible internal injury, severe laceration, or loss of consciousness." .


###  http://www.semanticweb.org/alecsculley/ontologies/2023/6/crimeontology#OWLClass_54e7b3be_15eb_418c_8ef9_2231d12c48dd
:OWLClass_54e7b3be_15eb_418c_8ef9_2231d12c48dd rdf:type owl:Class ;
                                               rdfs:subClassOf :OWLClass_6700c269_d438_4dcd_aa44_fda517de5744 ;
                                               rdfs:isDefinedBy "https://bjs.ojp.gov/sites/g/files/xyckuh236/files/sarble/data_common/nibrs-user-manual-2021-1041521.pdf" ;
                                               rdfs:label "Export Violation"@en ;
                                               <http://www.w3.org/2004/02/skos/core#definition> "To knowingly or willfully defraud the United States by smuggling, exporting, or clandestinely distributing merchandise that should have been invoiced, received, bought, sold, or facilitate the transportation, the concealment, or sale of such merchandise after exportation." .


###  http://www.semanticweb.org/alecsculley/ontologies/2023/6/crimeontology#OWLClass_5652f57c_0f7a_4861_9d4d_1f869b515893
:OWLClass_5652f57c_0f7a_4861_9d4d_1f869b515893 rdf:type owl:Class ;
                                               rdfs:subClassOf :OWLClass_88536041_a2e5_48a7_8cd1_a21b8217d6e6 ;
                                               rdfs:isDefinedBy "https://bjs.ojp.gov/sites/g/files/xyckuh236/files/sarble/data_common/nibrs-user-manual-2021-1041521.pdf" ;
                                               rdfs:label "Flight to Avoid Prosecution"@en ;
                                               <http://www.w3.org/2004/02/skos/core#definition> "To knowingly leave the jurisdiction where charges were filed with intent to avoid prosecution, custody, confinement, or to avoid giving testimony in any criminal proceedings." .


###  http://www.semanticweb.org/alecsculley/ontologies/2023/6/crimeontology#OWLClass_580ef448_2636_451a_8f5f_0a712a4d150c
:OWLClass_580ef448_2636_451a_8f5f_0a712a4d150c rdf:type owl:Class ;
                                               rdfs:subClassOf :OWLClass_9228dce9_8e81_499c_bba6_734e52015fdb ;
                                               owl:disjointWith :OWLClass_b1757863_d7f4_42a1_bb84_2787a39e91e5 ;
                                               rdfs:isDefinedBy "https://bjs.ojp.gov/sites/g/files/xyckuh236/files/sarble/data_common/nibrs-user-manual-2021-1041521.pdf" ;
                                               rdfs:label "Human Trafficking, Commercial Sex Act"@en ;
                                               <http://www.w3.org/2004/02/skos/core#definition> "Inducing a person by force, fraud, or coercion to participate in commercial sex acts, or in which the person induced to perform such act(s) has not attained 18 years of age." .


###  http://www.semanticweb.org/alecsculley/ontologies/2023/6/crimeontology#OWLClass_58bb6dd1_e6da_4afd_bd80_ccb657c2a56b
:OWLClass_58bb6dd1_e6da_4afd_bd80_ccb657c2a56b rdf:type owl:Class ;
                                               rdfs:subClassOf <http://purl.obolibrary.org/obo/BFO_0000015> ;
                                               rdfs:label "Criminal Incident"@en .


###  http://www.semanticweb.org/alecsculley/ontologies/2023/6/crimeontology#OWLClass_625939c9_9afe_4c33_ada6_f2226dfcd0d4
:OWLClass_625939c9_9afe_4c33_ada6_f2226dfcd0d4 rdf:type owl:Class ;
                                               rdfs:subClassOf :OWLClass_09a1351d_0eae_43fd_8841_989b08e40a54 ;
                                               rdfs:comment "NIBRS 2021 says this is a sex offense, but there is no sexual act involved in this offense. So, it is not a sex offense." ;
                                               rdfs:isDefinedBy "https://bjs.ojp.gov/sites/g/files/xyckuh236/files/sarble/data_common/nibrs-user-manual-2021-1041521.pdf" ;
                                               rdfs:label "Failure to Register as a Sex Offender"@en ;
                                               <http://www.w3.org/2004/02/skos/core#definition> "To fail to register or keep current a registration as required by state and federal laws." .


###  http://www.semanticweb.org/alecsculley/ontologies/2023/6/crimeontology#OWLClass_66b2c552_1100_423c_999a_338135d8df36
:OWLClass_66b2c552_1100_423c_999a_338135d8df36 rdf:type owl:Class ;
                                               rdfs:subClassOf :OWLClass_09a1351d_0eae_43fd_8841_989b08e40a54 ;
                                               rdfs:isDefinedBy "https://bjs.ojp.gov/sites/g/files/xyckuh236/files/sarble/data_common/nibrs-user-manual-2021-1041521.pdf" ;
                                               rdfs:label "Animal Cruelty"@en ;
                                               <http://www.w3.org/2004/02/skos/core#definition> "Intentionally, knowingly, or recklessly taking an action that mistreats or kills any animal without just cause, such as torturing, tormenting, mutilation, maiming, poisoning, or abandonment. Included are instances of duty to provide care, e.g., shelter, food, water, care if sick or injured; transporting or confining an animal to fight with another; inflicting excessive or repeated unnecessary pain or suffering, e.g., uses objects to beat or injure an animal. This definition does not include proper maintenance of animals for show or sport; use of animals for food, lawful hunting, fishing or trapping." .


###  http://www.semanticweb.org/alecsculley/ontologies/2023/6/crimeontology#OWLClass_6700c269_d438_4dcd_aa44_fda517de5744
:OWLClass_6700c269_d438_4dcd_aa44_fda517de5744 rdf:type owl:Class ;
                                               rdfs:subClassOf :OWLClass_09a1351d_0eae_43fd_8841_989b08e40a54 ;
                                               rdfs:isDefinedBy "https://bjs.ojp.gov/sites/g/files/xyckuh236/files/sarble/data_common/nibrs-user-manual-2021-1041521.pdf" ;
                                               rdfs:label "Commerce Violation"@en .


###  http://www.semanticweb.org/alecsculley/ontologies/2023/6/crimeontology#OWLClass_67484d5f_e3b4_4218_bb7e_b39f4a765918
:OWLClass_67484d5f_e3b4_4218_bb7e_b39f4a765918 rdf:type owl:Class ;
                                               rdfs:subClassOf :OWLClass_bc6631dd_6969_4e1a_9221_1eb96781d318 ;
                                               rdfs:isDefinedBy "https://bjs.ojp.gov/sites/g/files/xyckuh236/files/sarble/data_common/nibrs-user-manual-2021-1041521.pdf" ;
                                               rdfs:label "Arson"@en ;
                                               <http://www.w3.org/2004/02/skos/core#definition> "To unlawfully and intentionally damage or attempt to damage any real or personal property of another person or entity by fire or incendiary device." .


###  http://www.semanticweb.org/alecsculley/ontologies/2023/6/crimeontology#OWLClass_698463f0_cc06_4dac_849e_c7c3da22d3f2
:OWLClass_698463f0_cc06_4dac_849e_c7c3da22d3f2 rdf:type owl:Class ;
                                               rdfs:subClassOf :OWLClass_7a3cf11d_bd4a_475d_a5a3_9cd5b5e015b4 ;
                                               rdfs:isDefinedBy "https://bjs.ojp.gov/sites/g/files/xyckuh236/files/sarble/data_common/nibrs-user-manual-2021-1041521.pdf" ;
                                               rdfs:label "Aggravated Assault"@en ;
                                               <http://www.w3.org/2004/02/skos/core#definition> "An unlawful attack by one person upon another wherein the offender uses a dangerous weapon or displays it in a threatening manner or the victim suffers obvious severe or aggravated bodily injury, or where there was a risk for serious injury/intent to seriously injure." .


###  http://www.semanticweb.org/alecsculley/ontologies/2023/6/crimeontology#OWLClass_698d3768_6ed4_4042_88af_0f05dc222535
:OWLClass_698d3768_6ed4_4042_88af_0f05dc222535 rdf:type owl:Class ;
                                               rdfs:subClassOf <http://purl.obolibrary.org/obo/BFO_0000015> ;
                                               rdfs:label "Crime"@en ;
                                               <http://www.w3.org/2004/02/skos/core#definition> "A crime is an act that some law prescribes as punishable." .


###  http://www.semanticweb.org/alecsculley/ontologies/2023/6/crimeontology#OWLClass_6c5db9b0_ca24_4dc8_8a65_b67ce9dd6f49
:OWLClass_6c5db9b0_ca24_4dc8_8a65_b67ce9dd6f49 rdf:type owl:Class ;
                                               rdfs:subClassOf :OWLClass_ffc3cd08_93aa_46ec_819c_ba6a08344509 ;
                                               rdfs:isDefinedBy "https://bjs.ojp.gov/sites/g/files/xyckuh236/files/sarble/data_common/nibrs-user-manual-2021-1041521.pdf" ;
                                               rdfs:label "Shoplifting"@en ;
                                               <http://www.w3.org/2004/02/skos/core#definition> "The unlawful taking of goods or merchandise exposed for sale by a person (other than an employee)." .


###  http://www.semanticweb.org/alecsculley/ontologies/2023/6/crimeontology#OWLClass_6f059cff_9014_461c_a1d3_1aef83dc32f6
:OWLClass_6f059cff_9014_461c_a1d3_1aef83dc32f6 rdf:type owl:Class ;
                                               rdfs:subClassOf :OWLClass_ffc3cd08_93aa_46ec_819c_ba6a08344509 ;
                                               rdfs:isDefinedBy "https://bjs.ojp.gov/sites/g/files/xyckuh236/files/sarble/data_common/nibrs-user-manual-2021-1041521.pdf" ;
                                               rdfs:label "Theft from Coin-Operated Machine or Device"@en ;
                                               <http://www.w3.org/2004/02/skos/core#definition> "The unlawful taking of items from a machine or device that is operated or activated by the use of coins." .


###  http://www.semanticweb.org/alecsculley/ontologies/2023/6/crimeontology#OWLClass_71372462_77ce_4168_b7a2_6ecccf9aa3ff
:OWLClass_71372462_77ce_4168_b7a2_6ecccf9aa3ff rdf:type owl:Class ;
                                               rdfs:subClassOf :OWLClass_468582e8_7bed_4d62_816b_aca1037cec5c ;
                                               rdfs:isDefinedBy "https://bjs.ojp.gov/sites/g/files/xyckuh236/files/sarble/data_common/nibrs-user-manual-2021-1041521.pdf" ;
                                               rdfs:label "Fondling"@en ;
                                               <http://www.w3.org/2004/02/skos/core#definition> "The touching of the private body parts of another person for the purpose of sexual gratification, without the consent of the victim, including instances where the victim is unable to give consent because of his/her age or because of his/her temporary or permanent mental or physical incapacity." .


###  http://www.semanticweb.org/alecsculley/ontologies/2023/6/crimeontology#OWLClass_7229b7cb_15aa_41db_94ea_f7957964f0b2
:OWLClass_7229b7cb_15aa_41db_94ea_f7957964f0b2 rdf:type owl:Class ;
                                               rdfs:subClassOf :OWLClass_d6aabe44_4c76_4912_b4ee_6ff6278fa214 ;
                                               rdfs:isDefinedBy "https://bjs.ojp.gov/sites/g/files/xyckuh236/files/sarble/data_common/nibrs-user-manual-2021-1041521.pdf" ;
                                               rdfs:label "False Pretenses/Swindle/Confidence Game"@en ;
                                               <http://www.w3.org/2004/02/skos/core#definition> "The intentional misrepresentation of existing fact or condition or the use of some other deceptive scheme or device to obtain money, goods, or other things of value. Only includes fraud offenses that do not fit any of the definitions of the specific subcategories of fraud." .


###  http://www.semanticweb.org/alecsculley/ontologies/2023/6/crimeontology#OWLClass_7a3cf11d_bd4a_475d_a5a3_9cd5b5e015b4
:OWLClass_7a3cf11d_bd4a_475d_a5a3_9cd5b5e015b4 rdf:type owl:Class ;
                                               rdfs:subClassOf :OWLClass_4a556836_abaa_4c4b_93ae_bceaed442c48 ;
                                               rdfs:isDefinedBy "https://bjs.ojp.gov/sites/g/files/xyckuh236/files/sarble/data_common/nibrs-user-manual-2021-1041521.pdf" ;
                                               rdfs:label "Assault Offense"@en ;
                                               <http://www.w3.org/2004/02/skos/core#definition> "An unlawful attack by one person upon another." .


###  http://www.semanticweb.org/alecsculley/ontologies/2023/6/crimeontology#OWLClass_7accaf83_8383_41d4_be07_23b4bb44c264
:OWLClass_7accaf83_8383_41d4_be07_23b4bb44c264 rdf:type owl:Class ;
                                               rdfs:subClassOf :OWLClass_a8a577c3_d157_42d4_bd84_b53f80c7044c ;
                                               rdfs:isDefinedBy "https://bjs.ojp.gov/sites/g/files/xyckuh236/files/sarble/data_common/nibrs-user-manual-2021-1041521.pdf" ;
                                               rdfs:label "Explosives Violation"@en ;
                                               <http://www.w3.org/2004/02/skos/core#definition> "To knowingly violate the federal law prohibiting the manufacture, importation, sale, purchases, transfer, possession, unlawful use, intra or interstate transportation, or improper storage of any chemical compound mixture the primary or common purpose of which is to function by explosion including explosive materials or any explosive bomb, rocket, grenade, missile, or similar device, or any incendiary bomb or grenade, fire bomb, or “Molotov cocktail”." .


###  http://www.semanticweb.org/alecsculley/ontologies/2023/6/crimeontology#OWLClass_7ea8e635_5c0c_47b8_849a_6905d5ba4e72
:OWLClass_7ea8e635_5c0c_47b8_849a_6905d5ba4e72 rdf:type owl:Class ;
                                               rdfs:subClassOf :OWLClass_bc6631dd_6969_4e1a_9221_1eb96781d318 ;
                                               rdfs:isDefinedBy "https://bjs.ojp.gov/sites/g/files/xyckuh236/files/sarble/data_common/nibrs-user-manual-2021-1041521.pdf" ;
                                               rdfs:label "Embezzlement"@en ;
                                               <http://www.w3.org/2004/02/skos/core#definition> "The unlawful misappropriation by an offender to his/her own use or purpose of money, property, or some other thing of value entrusted to his/her care, custody, or control." .


###  http://www.semanticweb.org/alecsculley/ontologies/2023/6/crimeontology#OWLClass_7fae1cfd_c75e_4aa7_8873_09e0af238e91
:OWLClass_7fae1cfd_c75e_4aa7_8873_09e0af238e91 rdf:type owl:Class ;
                                               rdfs:subClassOf :OWLClass_93dc2b9e_a62b_4559_a478_fbffa91737ca ;
                                               rdfs:isDefinedBy "https://bjs.ojp.gov/sites/g/files/xyckuh236/files/sarble/data_common/nibrs-user-manual-2021-1041521.pdf" ;
                                               rdfs:label "Purchasing Prostitution"@en ;
                                               <http://www.w3.org/2004/02/skos/core#definition> "To purchase or trade anything of value for sex acts." .


###  http://www.semanticweb.org/alecsculley/ontologies/2023/6/crimeontology#OWLClass_804f0e44_5827_4635_a749_086d1bbdd1be
:OWLClass_804f0e44_5827_4635_a749_086d1bbdd1be rdf:type owl:Class ;
                                               rdfs:subClassOf :OWLClass_d6aabe44_4c76_4912_b4ee_6ff6278fa214 ;
                                               rdfs:isDefinedBy "https://bjs.ojp.gov/sites/g/files/xyckuh236/files/sarble/data_common/nibrs-user-manual-2021-1041521.pdf" ;
                                               rdfs:label "Welfare Fraud"@en ;
                                               <http://www.w3.org/2004/02/skos/core#definition> "The use of deceitful statements, practices, or devices to unlawfully obtain welfare benefits." .


###  http://www.semanticweb.org/alecsculley/ontologies/2023/6/crimeontology#OWLClass_807d4860_2bd2_49dc_9753_c60943e7217f
:OWLClass_807d4860_2bd2_49dc_9753_c60943e7217f rdf:type owl:Class ;
                                               rdfs:subClassOf :OWLClass_bc6631dd_6969_4e1a_9221_1eb96781d318 ;
                                               rdfs:isDefinedBy "https://bjs.ojp.gov/sites/g/files/xyckuh236/files/sarble/data_common/nibrs-user-manual-2021-1041521.pdf" ;
                                               rdfs:label "Stolen Property Offense"@en ;
                                               <http://www.w3.org/2004/02/skos/core#definition> "Buying, receiving, possessing, selling, concealing, or transporting any property with the knowledge that it has been unlawfully taken, as by burglary, embezzlement, fraud, larceny, robbery, etc." .


###  http://www.semanticweb.org/alecsculley/ontologies/2023/6/crimeontology#OWLClass_8703501d_4e88_42a5_9e84_80390e4b086a
:OWLClass_8703501d_4e88_42a5_9e84_80390e4b086a rdf:type owl:Class ;
                                               rdfs:subClassOf :OWLClass_6700c269_d438_4dcd_aa44_fda517de5744 ;
                                               rdfs:isDefinedBy "https://bjs.ojp.gov/sites/g/files/xyckuh236/files/sarble/data_common/nibrs-user-manual-2021-1041521.pdf" ;
                                               rdfs:label "Import Violation"@en ;
                                               <http://www.w3.org/2004/02/skos/core#definition> "To knowingly or willfully defraud the United States by smuggling, importing, or clandestinely introducing merchandise that should have been invoiced, received, bought, sold, or facilitate the transportation, the concealment, or sale of such merchandise after importation." .


###  http://www.semanticweb.org/alecsculley/ontologies/2023/6/crimeontology#OWLClass_871571d9_8a8d_4c1b_b0ab_9185f8d1e539
:OWLClass_871571d9_8a8d_4c1b_b0ab_9185f8d1e539 rdf:type owl:Class ;
                                               rdfs:subClassOf :OWLClass_ffc3cd08_93aa_46ec_819c_ba6a08344509 ;
                                               rdfs:isDefinedBy "https://bjs.ojp.gov/sites/g/files/xyckuh236/files/sarble/data_common/nibrs-user-manual-2021-1041521.pdf" ;
                                               rdfs:label "Theft from Building"@en ;
                                               <http://www.w3.org/2004/02/skos/core#definition> "The unlawful taking of items from within a building which is either open to the general public or to which the offender has legal access." .


###  http://www.semanticweb.org/alecsculley/ontologies/2023/6/crimeontology#OWLClass_88536041_a2e5_48a7_8cd1_a21b8217d6e6
:OWLClass_88536041_a2e5_48a7_8cd1_a21b8217d6e6 rdf:type owl:Class ;
                                               rdfs:subClassOf :OWLClass_09a1351d_0eae_43fd_8841_989b08e40a54 ;
                                               rdfs:label "Fugitive Offense"@en .


###  http://www.semanticweb.org/alecsculley/ontologies/2023/6/crimeontology#OWLClass_8b9b67c8_10df_49c9_84f3_ff1e67104f6c
:OWLClass_8b9b67c8_10df_49c9_84f3_ff1e67104f6c rdf:type owl:Class ;
                                               rdfs:subClassOf :OWLClass_fabdd37c_04aa_4a14_bcc7_6a56bd65ffa4 ;
                                               rdfs:isDefinedBy "https://bjs.ojp.gov/sites/g/files/xyckuh236/files/sarble/data_common/nibrs-user-manual-2021-1041521.pdf" ;
                                               rdfs:label "Illegal Entry into the United States"@en ;
                                               <http://www.w3.org/2004/02/skos/core#definition> "To attempt to enter the U.S. at any time or place other than as designated; or eludes examination/inspection by immigration officers." .


###  http://www.semanticweb.org/alecsculley/ontologies/2023/6/crimeontology#OWLClass_8e4e42b3_e6f0_4fe0_b73c_2ce50423b569
:OWLClass_8e4e42b3_e6f0_4fe0_b73c_2ce50423b569 rdf:type owl:Class ;
                                               rdfs:subClassOf :OWLClass_468582e8_7bed_4d62_816b_aca1037cec5c ;
                                               rdfs:isDefinedBy "https://bjs.ojp.gov/sites/g/files/xyckuh236/files/sarble/data_common/nibrs-user-manual-2021-1041521.pdf" ;
                                               rdfs:label "Sexual Assault with an Object"@en ;
                                               <http://www.w3.org/2004/02/skos/core#definition> "To use an object or instrument to unlawfully penetrate, however slightly, the genital or anal opening of the body of another person, without the consent of the victim, including instances where the victim is unable to give consent because of his/her age or because of his/her temporary or permanent mental or physical incapacity." .


###  http://www.semanticweb.org/alecsculley/ontologies/2023/6/crimeontology#OWLClass_8fe478d3_b15d_4192_9a18_1318cce7ecb7
:OWLClass_8fe478d3_b15d_4192_9a18_1318cce7ecb7 rdf:type owl:Class ;
                                               rdfs:subClassOf :OWLClass_d6aabe44_4c76_4912_b4ee_6ff6278fa214 ;
                                               rdfs:isDefinedBy "https://bjs.ojp.gov/sites/g/files/xyckuh236/files/sarble/data_common/nibrs-user-manual-2021-1041521.pdf" ;
                                               rdfs:label "Impersonation"@en ;
                                               <http://www.w3.org/2004/02/skos/core#definition> "Unlawfully representing one’s position and acting in the character or position to deceive others and thereby gain a profit or advantage, or enjoy some right or privilege." .


###  http://www.semanticweb.org/alecsculley/ontologies/2023/6/crimeontology#OWLClass_9228dce9_8e81_499c_bba6_734e52015fdb
:OWLClass_9228dce9_8e81_499c_bba6_734e52015fdb rdf:type owl:Class ;
                                               rdfs:subClassOf :OWLClass_4a556836_abaa_4c4b_93ae_bceaed442c48 ;
                                               rdfs:isDefinedBy "https://bjs.ojp.gov/sites/g/files/xyckuh236/files/sarble/data_common/nibrs-user-manual-2021-1041521.pdf" ;
                                               rdfs:label "Human Trafficking"@en ;
                                               <http://www.w3.org/2004/02/skos/core#definition> "The inducement of a person to perform a commercial sex act, or labor, or services, through force, fraud, or coercion.  Human trafficking has also occurred if a person under 18 years of age has been induced, or enticed, regardless of force, fraud, or coercion, to perform a commercial sex act." .


###  http://www.semanticweb.org/alecsculley/ontologies/2023/6/crimeontology#OWLClass_9395e80f_b7df_4749_97a8_df6dbcbd297e
:OWLClass_9395e80f_b7df_4749_97a8_df6dbcbd297e rdf:type owl:Class ;
                                               rdfs:subClassOf :OWLClass_d6aabe44_4c76_4912_b4ee_6ff6278fa214 ;
                                               rdfs:isDefinedBy "https://bjs.ojp.gov/sites/g/files/xyckuh236/files/sarble/data_common/nibrs-user-manual-2021-1041521.pdf" ;
                                               rdfs:label "Hacking/Computer Invasion"@en ;
                                               <http://www.w3.org/2004/02/skos/core#definition> "Gaining access to another person’s or institution’s computer software, hardware, or networks without authorized permissions." .


###  http://www.semanticweb.org/alecsculley/ontologies/2023/6/crimeontology#OWLClass_93dc2b9e_a62b_4559_a478_fbffa91737ca
:OWLClass_93dc2b9e_a62b_4559_a478_fbffa91737ca rdf:type owl:Class ;
                                               rdfs:subClassOf :OWLClass_09a1351d_0eae_43fd_8841_989b08e40a54 ;
                                               rdfs:isDefinedBy "https://bjs.ojp.gov/sites/g/files/xyckuh236/files/sarble/data_common/nibrs-user-manual-2021-1041521.pdf" ;
                                               rdfs:label "Prostitution Offense"@en ;
                                               <http://www.w3.org/2004/02/skos/core#definition> "To unlawfully engage in or promote sexual activities for anything of value." .


###  http://www.semanticweb.org/alecsculley/ontologies/2023/6/crimeontology#OWLClass_962c7c6c_ffaa_4d9c_a656_bb339e4ff6cc
:OWLClass_962c7c6c_ffaa_4d9c_a656_bb339e4ff6cc rdf:type owl:Class ;
                                               rdfs:subClassOf :OWLClass_4a556836_abaa_4c4b_93ae_bceaed442c48 ;
                                               rdfs:isDefinedBy "https://bjs.ojp.gov/sites/g/files/xyckuh236/files/sarble/data_common/nibrs-user-manual-2021-1041521.pdf" ;
                                               rdfs:label "Kidnapping/Abduction"@en ;
                                               <http://www.w3.org/2004/02/skos/core#definition> "The unlawful seizure, transportation, and/or detention of a person against his/her will or of a minor without the consent of his/her custodial parent(s) or legal guardian." .


###  http://www.semanticweb.org/alecsculley/ontologies/2023/6/crimeontology#OWLClass_9c98f399_b2b1_46c3_918a_ebf40b1c4938
:OWLClass_9c98f399_b2b1_46c3_918a_ebf40b1c4938 rdf:type owl:Class ;
                                               rdfs:subClassOf :OWLClass_468582e8_7bed_4d62_816b_aca1037cec5c ;
                                               rdfs:isDefinedBy "https://bjs.ojp.gov/sites/g/files/xyckuh236/files/sarble/data_common/nibrs-user-manual-2021-1041521.pdf" ;
                                               rdfs:label "Statutory Rape"@en ;
                                               <http://www.w3.org/2004/02/skos/core#definition> "Nonforcible sexual intercourse with a person who is under the statutory age of consent." .


###  http://www.semanticweb.org/alecsculley/ontologies/2023/6/crimeontology#OWLClass_9d3bdf2a_ce23_4ae0_9835_b15f278a36c1
:OWLClass_9d3bdf2a_ce23_4ae0_9835_b15f278a36c1 rdf:type owl:Class ;
                                               rdfs:subClassOf :OWLClass_b3e5e274_46a8_4fe5_a1d2_f72c3fda9bf6 ;
                                               rdfs:isDefinedBy "https://bjs.ojp.gov/sites/g/files/xyckuh236/files/sarble/data_common/nibrs-user-manual-2021-1041521.pdf" ;
                                               rdfs:label "Operating/Promoting/Assisting Gambling"@en ;
                                               <http://www.w3.org/2004/02/skos/core#definition> "To unlawfully operate, promote, or assist in the operation of a game of chance, lottery, or other gambling activity." .


###  http://www.semanticweb.org/alecsculley/ontologies/2023/6/crimeontology#OWLClass_9df332ef_449f_4518_8a43_2c8b915cb916
:OWLClass_9df332ef_449f_4518_8a43_2c8b915cb916 rdf:type owl:Class ;
                                               rdfs:subClassOf :OWLClass_93dc2b9e_a62b_4559_a478_fbffa91737ca ;
                                               rdfs:isDefinedBy "https://bjs.ojp.gov/sites/g/files/xyckuh236/files/sarble/data_common/nibrs-user-manual-2021-1041521.pdf" ;
                                               rdfs:label "Assisting or Promoting Prostitution"@en ;
                                               <http://www.w3.org/2004/02/skos/core#definition> "To solicit customers or transport persons for prostitution purposes; to own, manage, or operate a dwelling or other establishment for the purpose of providing a place where prostitution is performed; or to otherwise assist or promote prostitution." .


###  http://www.semanticweb.org/alecsculley/ontologies/2023/6/crimeontology#OWLClass_9e9c120e_a14e_4458_b8a1_7a6ca94e8420
:OWLClass_9e9c120e_a14e_4458_b8a1_7a6ca94e8420 rdf:type owl:Class ;
                                               rdfs:subClassOf :OWLClass_468582e8_7bed_4d62_816b_aca1037cec5c ;
                                               rdfs:isDefinedBy "https://bjs.ojp.gov/sites/g/files/xyckuh236/files/sarble/data_common/nibrs-user-manual-2021-1041521.pdf" ;
                                               rdfs:label "Sodomy"@en ;
                                               <http://www.w3.org/2004/02/skos/core#definition> "Oral or anal sexual intercourse with another person, without the consent of the victim, including instances where the victim is unable to give consent because of his/her age or because of his/her temporary or permanent mental or physical incapacity." .


###  http://www.semanticweb.org/alecsculley/ontologies/2023/6/crimeontology#OWLClass_a0c11abd_486f_4bbc_9ca7_91ed17448e76
:OWLClass_a0c11abd_486f_4bbc_9ca7_91ed17448e76 rdf:type owl:Class ;
                                               rdfs:subClassOf :OWLClass_ffc3cd08_93aa_46ec_819c_ba6a08344509 ;
                                               rdfs:isDefinedBy "https://bjs.ojp.gov/sites/g/files/xyckuh236/files/sarble/data_common/nibrs-user-manual-2021-1041521.pdf" ;
                                               rdfs:label "Theft of Motor Vehicle Parts or Accessories"@en ;
                                               <http://www.w3.org/2004/02/skos/core#definition> "The unlawful taking of any part or accessory affixed to the interior or exterior of a motor vehicle in a manner which would make the item an attachment of the vehicle or necessary for its operation." .


###  http://www.semanticweb.org/alecsculley/ontologies/2023/6/crimeontology#OWLClass_a8a577c3_d157_42d4_bd84_b53f80c7044c
:OWLClass_a8a577c3_d157_42d4_bd84_b53f80c7044c rdf:type owl:Class ;
                                               rdfs:subClassOf :OWLClass_09a1351d_0eae_43fd_8841_989b08e40a54 ;
                                               rdfs:isDefinedBy "https://bjs.ojp.gov/sites/g/files/xyckuh236/files/sarble/data_common/nibrs-user-manual-2021-1041521.pdf" ;
                                               rdfs:label "Weapon Law Violation"@en ;
                                               <http://www.w3.org/2004/02/skos/core#definition> "The violation of laws or ordinances prohibiting the manufacture, sale, purchase, transportation, possession, concealment, or use of firearms, cutting instruments, explosives, incendiary devices, or other deadly weapons." .


###  http://www.semanticweb.org/alecsculley/ontologies/2023/6/crimeontology#OWLClass_ab1951b1_39ec_4ccc_af50_2a3e76f9b5ed
:OWLClass_ab1951b1_39ec_4ccc_af50_2a3e76f9b5ed rdf:type owl:Class ;
                                               rdfs:subClassOf :OWLClass_4a556836_abaa_4c4b_93ae_bceaed442c48 ;
                                               rdfs:isDefinedBy "https://bjs.ojp.gov/sites/g/files/xyckuh236/files/sarble/data_common/nibrs-user-manual-2021-1041521.pdf" ;
                                               rdfs:label "Homicide Offense"@en ;
                                               <http://www.w3.org/2004/02/skos/core#definition> "The killing of one human being by another." .


###  http://www.semanticweb.org/alecsculley/ontologies/2023/6/crimeontology#OWLClass_ab2655b2_ef69_42aa_8fea_50047d1065ee
:OWLClass_ab2655b2_ef69_42aa_8fea_50047d1065ee rdf:type owl:Class ;
                                               rdfs:subClassOf :OWLClass_7a3cf11d_bd4a_475d_a5a3_9cd5b5e015b4 ;
                                               rdfs:isDefinedBy "https://bjs.ojp.gov/sites/g/files/xyckuh236/files/sarble/data_common/nibrs-user-manual-2021-1041521.pdf" ;
                                               rdfs:label "Intimidation"@en ;
                                               <http://www.w3.org/2004/02/skos/core#definition> "To unlawfully place another person in reasonable fear of harm through the use of threatening words and/or other conduct without displaying a dangerous weapon or subjecting the victim to an actual physical attack." .


###  http://www.semanticweb.org/alecsculley/ontologies/2023/6/crimeontology#OWLClass_b0a545cf_bb58_4aaa_bbac_bbe7d13260af
:OWLClass_b0a545cf_bb58_4aaa_bbac_bbe7d13260af rdf:type owl:Class ;
                                               rdfs:subClassOf :OWLClass_b3e5e274_46a8_4fe5_a1d2_f72c3fda9bf6 ;
                                               rdfs:isDefinedBy "https://bjs.ojp.gov/sites/g/files/xyckuh236/files/sarble/data_common/nibrs-user-manual-2021-1041521.pdf" ;
                                               rdfs:label "Sports Tampering"@en ;
                                               <http://www.w3.org/2004/02/skos/core#definition> "To unlawfully alter, meddle in, or otherwise interfere with a sporting contest or event for the purpose of gaining a gambling advantage." .


###  http://www.semanticweb.org/alecsculley/ontologies/2023/6/crimeontology#OWLClass_b1757863_d7f4_42a1_bb84_2787a39e91e5
:OWLClass_b1757863_d7f4_42a1_bb84_2787a39e91e5 rdf:type owl:Class ;
                                               rdfs:subClassOf :OWLClass_9228dce9_8e81_499c_bba6_734e52015fdb ;
                                               rdfs:isDefinedBy "https://bjs.ojp.gov/sites/g/files/xyckuh236/files/sarble/data_common/nibrs-user-manual-2021-1041521.pdf" ;
                                               rdfs:label "Human Trafficking, Involuntary Servitude"@en ;
                                               <http://www.w3.org/2004/02/skos/core#definition> "The obtaining of person(s) through recruitment, harboring, transportation, or provision, and subjecting such persons by force, fraud, or coercion into involuntary servitude, peonage, debt bondage, or slavery (not to include commercial sex acts)." .


###  http://www.semanticweb.org/alecsculley/ontologies/2023/6/crimeontology#OWLClass_b3e5e274_46a8_4fe5_a1d2_f72c3fda9bf6
:OWLClass_b3e5e274_46a8_4fe5_a1d2_f72c3fda9bf6 rdf:type owl:Class ;
                                               rdfs:subClassOf :OWLClass_09a1351d_0eae_43fd_8841_989b08e40a54 ;
                                               rdfs:isDefinedBy "https://bjs.ojp.gov/sites/g/files/xyckuh236/files/sarble/data_common/nibrs-user-manual-2021-1041521.pdf" ;
                                               rdfs:label "Gambling Offenses"@en ;
                                               <http://www.w3.org/2004/02/skos/core#definition> "To unlawfully bet or wager money or something else of value; assist, promote, or operate a game of chance for money or some other stake; possess or transmit wagering information; manufacture, sell, purchase, possess, or transport gambling equipment, devices, or goods; or tamper with the outcome of a sporting event or contest to gain a gambling advantage." .


###  http://www.semanticweb.org/alecsculley/ontologies/2023/6/crimeontology#OWLClass_b57af5d8_3242_4a76_9d87_a44f2a0b2348
:OWLClass_b57af5d8_3242_4a76_9d87_a44f2a0b2348 rdf:type owl:Class ;
                                               rdfs:subClassOf :OWLClass_09a1351d_0eae_43fd_8841_989b08e40a54 ;
                                               rdfs:isDefinedBy "https://bjs.ojp.gov/sites/g/files/xyckuh236/files/sarble/data_common/nibrs-user-manual-2021-1041521.pdf" ;
                                               rdfs:label "Treason"@en ;
                                               <http://www.w3.org/2004/02/skos/core#definition> "Whoever, owing allegiance to the United States, levies war against them or adheres to their enemies, giving them aid and comfort within the United States or elsewhere." .


###  http://www.semanticweb.org/alecsculley/ontologies/2023/6/crimeontology#OWLClass_b9d76e86_a9f3_4a44_b9ff_08d98c1750a4
:OWLClass_b9d76e86_a9f3_4a44_b9ff_08d98c1750a4 rdf:type owl:Class ;
                                               rdfs:subClassOf :OWLClass_ffc3cd08_93aa_46ec_819c_ba6a08344509 ;
                                               rdfs:isDefinedBy "https://bjs.ojp.gov/sites/g/files/xyckuh236/files/sarble/data_common/nibrs-user-manual-2021-1041521.pdf" ;
                                               rdfs:label "Purse-snatching"@en ;
                                               <http://www.w3.org/2004/02/skos/core#definition> "The grabbing or snatching of a purse, handbag, etc., from the physical possession of another person." .


###  http://www.semanticweb.org/alecsculley/ontologies/2023/6/crimeontology#OWLClass_ba7f835e_2039_4234_a7d6_188cc25f539f
:OWLClass_ba7f835e_2039_4234_a7d6_188cc25f539f rdf:type owl:Class ;
                                               rdfs:subClassOf :OWLClass_bc6631dd_6969_4e1a_9221_1eb96781d318 ;
                                               rdfs:isDefinedBy "https://bjs.ojp.gov/sites/g/files/xyckuh236/files/sarble/data_common/nibrs-user-manual-2021-1041521.pdf" ;
                                               rdfs:label "Bribery"@en ;
                                               <http://www.w3.org/2004/02/skos/core#definition> "The offering, giving, receiving, or soliciting anything of value (e.g., a bribe, gratuity, or kickback) to sway the judgement or action of a person in a position of trust or influence." .


###  http://www.semanticweb.org/alecsculley/ontologies/2023/6/crimeontology#OWLClass_bc6631dd_6969_4e1a_9221_1eb96781d318
:OWLClass_bc6631dd_6969_4e1a_9221_1eb96781d318 rdf:type owl:Class ;
                                               rdfs:subClassOf :OWLClass_698d3768_6ed4_4042_88af_0f05dc222535 ;
                                               <http://www.ontologyrepository.com/CommonCoreOntologies/definition_source> "https://bjs.ojp.gov/sites/g/files/xyckuh236/files/sarble/data_common/nibrs-user-manual-2021-1041521.pdf" ;
                                               rdfs:label "Crime Against Property"@en ;
                                               <http://www.w3.org/2004/02/skos/core#definition> "A crime against property is a crime that has the objective to obtain money, property, or some other benefit." .


###  http://www.semanticweb.org/alecsculley/ontologies/2023/6/crimeontology#OWLClass_bcf2ae10_def5_4957_9f8f_8a50bc2dbb2a
:OWLClass_bcf2ae10_def5_4957_9f8f_8a50bc2dbb2a rdf:type owl:Class ;
                                               rdfs:subClassOf :OWLClass_d6aabe44_4c76_4912_b4ee_6ff6278fa214 ;
                                               rdfs:isDefinedBy "https://bjs.ojp.gov/sites/g/files/xyckuh236/files/sarble/data_common/nibrs-user-manual-2021-1041521.pdf" ;
                                               rdfs:label "Credit Card/Automated Teller Machine Fraud"@en ;
                                               <http://www.w3.org/2004/02/skos/core#definition> "The unlawful use of a credit/debit card, credit/debit card number, or automatic teller machine for fraudulent purposes." .


###  http://www.semanticweb.org/alecsculley/ontologies/2023/6/crimeontology#OWLClass_bf5140fe_3913_4fa1_ad2f_cf72c98b3a1f
:OWLClass_bf5140fe_3913_4fa1_ad2f_cf72c98b3a1f rdf:type owl:Class ;
                                               rdfs:subClassOf :OWLClass_fabdd37c_04aa_4a14_bcc7_6a56bd65ffa4 ;
                                               rdfs:isDefinedBy "https://bjs.ojp.gov/sites/g/files/xyckuh236/files/sarble/data_common/nibrs-user-manual-2021-1041521.pdf" ;
                                               rdfs:label "Smuggling Aliens"@en ;
                                               <http://www.w3.org/2004/02/skos/core#definition> "To knowingly assist, abet, or aid another person to enter, or try to enter, the United States illegally." .


###  http://www.semanticweb.org/alecsculley/ontologies/2023/6/crimeontology#OWLClass_bfc89447_dbd1_4b11_b6d8_35eb20c16616
:OWLClass_bfc89447_dbd1_4b11_b6d8_35eb20c16616 rdf:type owl:Class ;
                                               rdfs:subClassOf :OWLClass_ffc3cd08_93aa_46ec_819c_ba6a08344509 ;
                                               rdfs:isDefinedBy "https://bjs.ojp.gov/sites/g/files/xyckuh236/files/sarble/data_common/nibrs-user-manual-2021-1041521.pdf" ;
                                               rdfs:label "All Other Larceny"@en ;
                                               <http://www.w3.org/2004/02/skos/core#definition> "All thefts which do not fit any of the Larceny/Theft or specific subcategories identified in UCR." .


###  http://www.semanticweb.org/alecsculley/ontologies/2023/6/crimeontology#OWLClass_c1a8c39d_2044_40c1_ba87_119c284acf3c
:OWLClass_c1a8c39d_2044_40c1_ba87_119c284acf3c rdf:type owl:Class ;
                                               rdfs:subClassOf :OWLClass_fabdd37c_04aa_4a14_bcc7_6a56bd65ffa4 ;
                                               rdfs:isDefinedBy "https://bjs.ojp.gov/sites/g/files/xyckuh236/files/sarble/data_common/nibrs-user-manual-2021-1041521.pdf" ;
                                               rdfs:label "Re-entry After Deportation"@en ;
                                               <http://www.w3.org/2004/02/skos/core#definition> "The act of entering, attempting to enter, or being found in the United States after being removed, excluded, deported, or has departed the United States while an order of removal exclusion or deportation is outstanding." .


###  http://www.semanticweb.org/alecsculley/ontologies/2023/6/crimeontology#OWLClass_c587f60d_3028_477e_979d_40fee70db23c
:OWLClass_c587f60d_3028_477e_979d_40fee70db23c rdf:type owl:Class ;
                                               rdfs:subClassOf :OWLClass_ab1951b1_39ec_4ccc_af50_2a3e76f9b5ed ;
                                               rdfs:isDefinedBy "https://bjs.ojp.gov/sites/g/files/xyckuh236/files/sarble/data_common/nibrs-user-manual-2021-1041521.pdf" ;
                                               rdfs:label "Negligent Manslaughter"@en ;
                                               <http://www.w3.org/2004/02/skos/core#definition> "The killing of another person through gross negligence." .


###  http://www.semanticweb.org/alecsculley/ontologies/2023/6/crimeontology#OWLClass_d13600f2_7687_4bbf_a075_3e20445663a8
:OWLClass_d13600f2_7687_4bbf_a075_3e20445663a8 rdf:type owl:Class ;
                                               rdfs:subClassOf :OWLClass_bc6631dd_6969_4e1a_9221_1eb96781d318 ;
                                               rdfs:isDefinedBy "https://bjs.ojp.gov/sites/g/files/xyckuh236/files/sarble/data_common/nibrs-user-manual-2021-1041521.pdf" ;
                                               rdfs:label "Motor Vehicle Theft"@en ;
                                               <http://www.w3.org/2004/02/skos/core#definition> "The theft of a motor vehicle." .


###  http://www.semanticweb.org/alecsculley/ontologies/2023/6/crimeontology#OWLClass_d2e735e5_9ab8_4c1a_a913_5e3ed0071439
:OWLClass_d2e735e5_9ab8_4c1a_a913_5e3ed0071439 rdf:type owl:Class ;
                                               rdfs:subClassOf :OWLClass_b3e5e274_46a8_4fe5_a1d2_f72c3fda9bf6 ;
                                               rdfs:isDefinedBy "https://bjs.ojp.gov/sites/g/files/xyckuh236/files/sarble/data_common/nibrs-user-manual-2021-1041521.pdf" ;
                                               rdfs:label "Betting/Wagering"@en ;
                                               <http://www.w3.org/2004/02/skos/core#definition> "To unlawfully stake money or something else of value on the happening of an uncertain event or on the ascertainment of a fact in dispute." .


###  http://www.semanticweb.org/alecsculley/ontologies/2023/6/crimeontology#OWLClass_d6aabe44_4c76_4912_b4ee_6ff6278fa214
:OWLClass_d6aabe44_4c76_4912_b4ee_6ff6278fa214 rdf:type owl:Class ;
                                               rdfs:subClassOf :OWLClass_bc6631dd_6969_4e1a_9221_1eb96781d318 ;
                                               rdfs:isDefinedBy "https://bjs.ojp.gov/sites/g/files/xyckuh236/files/sarble/data_common/nibrs-user-manual-2021-1041521.pdf" ;
                                               rdfs:label "Fraud Offense"@en ;
                                               <http://www.w3.org/2004/02/skos/core#definition> "The intentional perversion of the truth for the purpose of inducing another person or other entity in reliance upon it to part with something of value or to surrender a legal right." .


###  http://www.semanticweb.org/alecsculley/ontologies/2023/6/crimeontology#OWLClass_e1f6a4c6_30f2_4ad6_aeb6_ab9d4efdf45b
:OWLClass_e1f6a4c6_30f2_4ad6_aeb6_ab9d4efdf45b rdf:type owl:Class ;
                                               rdfs:subClassOf :OWLClass_a8a577c3_d157_42d4_bd84_b53f80c7044c ;
                                               rdfs:isDefinedBy "https://bjs.ojp.gov/sites/g/files/xyckuh236/files/sarble/data_common/nibrs-user-manual-2021-1041521.pdf" ;
                                               rdfs:label "Weapons of Mass Destruction Violation"@en ;
                                               <http://www.w3.org/2004/02/skos/core#definition> "To knowingly violate the federal law prohibiting the unlawful use, attempted use, conspiracy to use, or use of interstate travel or facilities in furtherance of the use of a weapon of mass destruction as defined by federal law." .


###  http://www.semanticweb.org/alecsculley/ontologies/2023/6/crimeontology#OWLClass_e21afa9c_e56e_46d3_9edd_6899c04ba2ee
:OWLClass_e21afa9c_e56e_46d3_9edd_6899c04ba2ee rdf:type owl:Class ;
                                               rdfs:subClassOf :OWLClass_6700c269_d438_4dcd_aa44_fda517de5744 ;
                                               rdfs:isDefinedBy "https://bjs.ojp.gov/sites/g/files/xyckuh236/files/sarble/data_common/nibrs-user-manual-2021-1041521.pdf" ;
                                               rdfs:label "Wildlife Trafficking"@en ;
                                               <http://www.w3.org/2004/02/skos/core#definition> "The poaching or other illegal taking of protected or managed species and the illegal trade in wildlife and their related parts and products." .


###  http://www.semanticweb.org/alecsculley/ontologies/2023/6/crimeontology#OWLClass_ed944433_c64e_4691_b5b6_2f687efd8fc0
:OWLClass_ed944433_c64e_4691_b5b6_2f687efd8fc0 rdf:type owl:Class ;
                                               rdfs:subClassOf :OWLClass_6700c269_d438_4dcd_aa44_fda517de5744 ;
                                               rdfs:isDefinedBy "https://bjs.ojp.gov/sites/g/files/xyckuh236/files/sarble/data_common/nibrs-user-manual-2021-1041521.pdf" ;
                                               rdfs:label "Federal Tobacco Offense"@en ;
                                               <http://www.w3.org/2004/02/skos/core#definition> "The unlawful possession and/or distribution of contraband tobacco products; including any quantity of cigarettes in excess of 10,000 or other tobacco products if the cigarettes/products bear no evidence of the payment of applicable state taxes in the state where the cigarettes are found.  Engaging in interstate commerce in tobacco products without registering with, and reporting to, the federal government and applicable state tax administrators." .


###  http://www.semanticweb.org/alecsculley/ontologies/2023/6/crimeontology#OWLClass_f3edd9ed_dcc9_4f65_a346_c4cc838c3d15
:OWLClass_f3edd9ed_dcc9_4f65_a346_c4cc838c3d15 rdf:type owl:Class ;
                                               rdfs:subClassOf :OWLClass_88536041_a2e5_48a7_8cd1_a21b8217d6e6 ;
                                               rdfs:isDefinedBy "https://bjs.ojp.gov/sites/g/files/xyckuh236/files/sarble/data_common/nibrs-user-manual-2021-1041521.pdf" ;
                                               rdfs:label "Flight to Aviod Deportation"@en ;
                                               <http://www.w3.org/2004/02/skos/core#definition> "To knowingly leave the jurisdiction with intent to avoid deportation." .


###  http://www.semanticweb.org/alecsculley/ontologies/2023/6/crimeontology#OWLClass_f4a0583f_8ccd_418d_ac06_8d39bf392843
:OWLClass_f4a0583f_8ccd_418d_ac06_8d39bf392843 rdf:type owl:Class ;
                                               rdfs:subClassOf :OWLClass_468582e8_7bed_4d62_816b_aca1037cec5c ;
                                               rdfs:isDefinedBy "https://bjs.ojp.gov/sites/g/files/xyckuh236/files/sarble/data_common/nibrs-user-manual-2021-1041521.pdf" ;
                                               rdfs:label "Rape"@en ;
                                               <http://www.w3.org/2004/02/skos/core#definition> "The carnal knowledge of a person, without the consent of the victim, including instances where the victim is unable to give consent because of his/her age or because of his/her temporary or permanent mental or physical incapacity." .


###  http://www.semanticweb.org/alecsculley/ontologies/2023/6/crimeontology#OWLClass_f8ff2fcb_ad53_4bfa_821e_36855e778a86
:OWLClass_f8ff2fcb_ad53_4bfa_821e_36855e778a86 rdf:type owl:Class ;
                                               rdfs:subClassOf :OWLClass_01941403_ff94_48f1_9377_c187032b4f53 ;
                                               rdfs:isDefinedBy "https://bjs.ojp.gov/sites/g/files/xyckuh236/files/sarble/data_common/nibrs-user-manual-2021-1041521.pdf" ;
                                               rdfs:label "Drug Equipment Violation"@en ;
                                               <http://www.w3.org/2004/02/skos/core#definition> "The unlawful manufacture, sale, purchase, possession, or transportation of equipment or devices utilized in preparing and/or using drugs or narcotics." .


###  http://www.semanticweb.org/alecsculley/ontologies/2023/6/crimeontology#OWLClass_fabdd37c_04aa_4a14_bcc7_6a56bd65ffa4
:OWLClass_fabdd37c_04aa_4a14_bcc7_6a56bd65ffa4 rdf:type owl:Class ;
                                               rdfs:subClassOf :OWLClass_09a1351d_0eae_43fd_8841_989b08e40a54 ;
                                               rdfs:label "Immigration Violation"@en .


###  http://www.semanticweb.org/alecsculley/ontologies/2023/6/crimeontology#OWLClass_ffc3cd08_93aa_46ec_819c_ba6a08344509
:OWLClass_ffc3cd08_93aa_46ec_819c_ba6a08344509 rdf:type owl:Class ;
                                               rdfs:subClassOf :OWLClass_bc6631dd_6969_4e1a_9221_1eb96781d318 ;
                                               rdfs:isDefinedBy "https://bjs.ojp.gov/sites/g/files/xyckuh236/files/sarble/data_common/nibrs-user-manual-2021-1041521.pdf" ;
                                               rdfs:label "Larceny/Theft Offense"@en ;
                                               <http://www.w3.org/2004/02/skos/core#definition> "The unlawful taking, carrying, leading, or riding away of property from the possession or constructive possession of another person." .


#################################################################
#    General axioms
#################################################################

[ rdf:type owl:AllDisjointClasses ;
  owl:members ( <http://purl.obolibrary.org/obo/BFO_0000182>
                :OWLClass_58bb6dd1_e6da_4afd_bd80_ccb657c2a56b
                :OWLClass_698d3768_6ed4_4042_88af_0f05dc222535
              )
] .


[ rdf:type owl:AllDisjointClasses ;
  owl:members ( :OWLClass_01a675dc_525d_402b_a75b_84002d5715ff
                :OWLClass_5652f57c_0f7a_4861_9d4d_1f869b515893
                :OWLClass_f3edd9ed_dcc9_4f65_a346_c4cc838c3d15
              )
] .


[ rdf:type owl:AllDisjointClasses ;
  owl:members ( :OWLClass_031abc3c_4c7c_4f2d_89d4_a17258417b93
                :OWLClass_22f2f59c_a6b7_412e_8ec1_d61cbeca0ce8
                :OWLClass_32d0d6a3_956a_4433_8b09_8f7d0febe84c
                :OWLClass_48331cbf_5784_4380_830b_a1aa865ed8ff
                :OWLClass_625939c9_9afe_4c33_ada6_f2226dfcd0d4
                :OWLClass_66b2c552_1100_423c_999a_338135d8df36
                :OWLClass_6700c269_d438_4dcd_aa44_fda517de5744
                :OWLClass_88536041_a2e5_48a7_8cd1_a21b8217d6e6
                :OWLClass_93dc2b9e_a62b_4559_a478_fbffa91737ca
                :OWLClass_a8a577c3_d157_42d4_bd84_b53f80c7044c
                :OWLClass_b3e5e274_46a8_4fe5_a1d2_f72c3fda9bf6
                :OWLClass_b57af5d8_3242_4a76_9d87_a44f2a0b2348
                :OWLClass_f8ff2fcb_ad53_4bfa_821e_36855e778a86
                :OWLClass_fabdd37c_04aa_4a14_bcc7_6a56bd65ffa4
              )
] .


[ rdf:type owl:AllDisjointClasses ;
  owl:members ( :OWLClass_04c8931b_7445_4b70_a44a_34563a22ef3b
                :OWLClass_3161b469_6ed6_4e04_bf54_33eb3df4b49b
                :OWLClass_7229b7cb_15aa_41db_94ea_f7957964f0b2
                :OWLClass_804f0e44_5827_4635_a749_086d1bbdd1be
                :OWLClass_8fe478d3_b15d_4192_9a18_1318cce7ecb7
                :OWLClass_9395e80f_b7df_4749_97a8_df6dbcbd297e
                :OWLClass_bcf2ae10_def5_4957_9f8f_8a50bc2dbb2a
              )
] .


[ rdf:type owl:AllDisjointClasses ;
  owl:members ( :OWLClass_0625c00d_9805_4639_9090_746645edcfde
                :OWLClass_54e7b3be_15eb_418c_8ef9_2231d12c48dd
                :OWLClass_8703501d_4e88_42a5_9e84_80390e4b086a
                :OWLClass_e21afa9c_e56e_46d3_9edd_6899c04ba2ee
                :OWLClass_ed944433_c64e_4691_b5b6_2f687efd8fc0
              )
] .


[ rdf:type owl:AllDisjointClasses ;
  owl:members ( :OWLClass_09a1351d_0eae_43fd_8841_989b08e40a54
                :OWLClass_4a556836_abaa_4c4b_93ae_bceaed442c48
                :OWLClass_bc6631dd_6969_4e1a_9221_1eb96781d318
              )
] .


[ rdf:type owl:AllDisjointClasses ;
  owl:members ( :OWLClass_0bdcbb40_9669_4246_8b85_44f5315a9cfa
                :OWLClass_7accaf83_8383_41d4_be07_23b4bb44c264
                :OWLClass_e1f6a4c6_30f2_4ad6_aeb6_ab9d4efdf45b
              )
] .


[ rdf:type owl:AllDisjointClasses ;
  owl:members ( :OWLClass_0be0fff2_6aac_44b7_af4e_d5708695a424
                :OWLClass_9d3bdf2a_ce23_4ae0_9835_b15f278a36c1
                :OWLClass_b0a545cf_bb58_4aaa_bbac_bbe7d13260af
                :OWLClass_d2e735e5_9ab8_4c1a_a913_5e3ed0071439
              )
] .


[ rdf:type owl:AllDisjointClasses ;
  owl:members ( :OWLClass_13a3be60_8fc3_45a2_bc5b_bc94f077bc6b
                :OWLClass_7fae1cfd_c75e_4aa7_8873_09e0af238e91
                :OWLClass_9df332ef_449f_4518_8a43_2c8b915cb916
              )
] .


[ rdf:type owl:AllDisjointClasses ;
  owl:members ( :OWLClass_20216fa3_d400_4d05_b118_db40fb8f01e4
                :OWLClass_8b9b67c8_10df_49c9_84f3_ff1e67104f6c
                :OWLClass_bf5140fe_3913_4fa1_ad2f_cf72c98b3a1f
                :OWLClass_c1a8c39d_2044_40c1_ba87_119c284acf3c
              )
] .


[ rdf:type owl:AllDisjointClasses ;
  owl:members ( :OWLClass_275c50da_46a5_4715_a4e0_b0f5406e9820
                :OWLClass_3384efaa_3631_49f6_831f_108b94381362
                :OWLClass_398810e4_2b87_40a1_9ba3_2059acb81322
                :OWLClass_3b713ed2_061e_496a_a6ca_bc924a3024eb
                :OWLClass_3ee541f8_ad76_4a09_bfe3_80e17b381f91
                :OWLClass_67484d5f_e3b4_4218_bb7e_b39f4a765918
                :OWLClass_7ea8e635_5c0c_47b8_849a_6905d5ba4e72
                :OWLClass_807d4860_2bd2_49dc_9753_c60943e7217f
                :OWLClass_ba7f835e_2039_4234_a7d6_188cc25f539f
                :OWLClass_d13600f2_7687_4bbf_a075_3e20445663a8
                :OWLClass_d6aabe44_4c76_4912_b4ee_6ff6278fa214
                :OWLClass_ffc3cd08_93aa_46ec_819c_ba6a08344509
              )
] .


[ rdf:type owl:AllDisjointClasses ;
  owl:members ( :OWLClass_2bf259d2_3ccc_4934_9b91_b6a3c2a73103
                :OWLClass_342e0730_c70f_4afa_909f_1c443bae77ac
                :OWLClass_6c5db9b0_ca24_4dc8_8a65_b67ce9dd6f49
                :OWLClass_6f059cff_9014_461c_a1d3_1aef83dc32f6
                :OWLClass_871571d9_8a8d_4c1b_b0ab_9185f8d1e539
                :OWLClass_a0c11abd_486f_4bbc_9ca7_91ed17448e76
                :OWLClass_b9d76e86_a9f3_4a44_b9ff_08d98c1750a4
                :OWLClass_bfc89447_dbd1_4b11_b6d8_35eb20c16616
              )
] .


[ rdf:type owl:AllDisjointClasses ;
  owl:members ( :OWLClass_3305dd81_545d_4750_afc8_9221881757f8
                :OWLClass_71372462_77ce_4168_b7a2_6ecccf9aa3ff
                :OWLClass_8e4e42b3_e6f0_4fe0_b73c_2ce50423b569
                :OWLClass_9c98f399_b2b1_46c3_918a_ebf40b1c4938
                :OWLClass_9e9c120e_a14e_4458_b8a1_7a6ca94e8420
                :OWLClass_f4a0583f_8ccd_418d_ac06_8d39bf392843
              )
] .


[ rdf:type owl:AllDisjointClasses ;
  owl:members ( :OWLClass_468582e8_7bed_4d62_816b_aca1037cec5c
                :OWLClass_7a3cf11d_bd4a_475d_a5a3_9cd5b5e015b4
                :OWLClass_9228dce9_8e81_499c_bba6_734e52015fdb
                :OWLClass_962c7c6c_ffaa_4d9c_a656_bb339e4ff6cc
                :OWLClass_ab1951b1_39ec_4ccc_af50_2a3e76f9b5ed
              )
] .


[ rdf:type owl:AllDisjointClasses ;
  owl:members ( :OWLClass_4b003f10_d59f_490b_91d9_6f2d122f6a5d
                :OWLClass_698463f0_cc06_4dac_849e_c7c3da22d3f2
                :OWLClass_ab2655b2_ef69_42aa_8fea_50047d1065ee
              )
] .


###  Generated by the OWL API (version 4.5.9.2019-02-01T07:24:44Z) https://github.com/owlcs/owlapi
