@prefix : <http://www.semanticweb.org/alecsculley/ontologies/crimeontology/> .
@prefix owl: <http://www.w3.org/2002/07/owl#> .
@prefix rdf: <http://www.w3.org/1999/02/22-rdf-syntax-ns#> .
@prefix xml: <http://www.w3.org/XML/1998/namespace> .
@prefix xsd: <http://www.w3.org/2001/XMLSchema#> .
@prefix rdfs: <http://www.w3.org/2000/01/rdf-schema#> .
@base <http://www.semanticweb.org/alecsculley/ontologies/crimeontology/> .

<http://www.semanticweb.org/alecsculley/ontologies/crimeontology/> rdf:type owl:Ontology ;
                                                                    owl:imports <http://purl.obolibrary.org/obo/1.0.0/bfo-core.owl> .

#################################################################
#    Annotation properties
#################################################################

###  http://purl.org/dc/elements/1.1/creator
<http://purl.org/dc/elements/1.1/creator> rdf:type owl:AnnotationProperty .


###  http://www.ontologyrepository.com/CommonCoreOntologies/definition
<http://www.ontologyrepository.com/CommonCoreOntologies/definition> rdf:type owl:AnnotationProperty .


###  http://www.ontologyrepository.com/CommonCoreOntologies/definition_source
<http://www.ontologyrepository.com/CommonCoreOntologies/definition_source> rdf:type owl:AnnotationProperty .


###  http://www.ontologyrepository.com/CommonCoreOntologies/is_curated_in_ontology
<http://www.ontologyrepository.com/CommonCoreOntologies/is_curated_in_ontology> rdf:type owl:AnnotationProperty .


#################################################################
#    Classes
#################################################################

###  http://www.ontologyrepository.com/CommonCoreOntologies/Act
<http://www.ontologyrepository.com/CommonCoreOntologies/Act> rdf:type owl:Class ;
                                                             rdfs:subClassOf <http://purl.obolibrary.org/obo/BFO_0000015> ;
                                                             <http://www.ontologyrepository.com/CommonCoreOntologies/definition> "A Process in which at least one Agent plays a causative role."@en ;
                                                             <http://www.ontologyrepository.com/CommonCoreOntologies/is_curated_in_ontology> "http://www.ontologyrepository.com/CommonCoreOntologies/Mid/EventOntology"^^xsd:anyURI ;
                                                             rdfs:label "Act"@en .


###  http://www.semanticweb.org/alecsculley/ontologies/crimeontology/CrO_0000006
:CrO_0000006 rdf:type owl:Class ;
                    rdfs:subClassOf :CrO_0000009 ;
                    rdfs:isDefinedBy "https://bjs.ojp.gov/sites/g/files/xyckuh236/files/sarble/data_common/nibrs-user-manual-2021-1041521.pdf" ;
                    rdfs:label "Aggravated Assault"@en ;
                    <http://www.w3.org/2004/02/skos/core#definition> "An unlawful attack by one person upon another wherein the offender uses a dangerous weapon or displays it in a threatening manner or the victim suffers obvious severe or aggravated bodily injury, or where there was a risk for serious injury/intent to seriously injure." .


###  http://www.semanticweb.org/alecsculley/ontologies/crimeontology/CrO_0000007
:CrO_0000007 rdf:type owl:Class ;
                rdfs:subClassOf :CrO_0000005 ;
                rdfs:isDefinedBy "https://bjs.ojp.gov/sites/g/files/xyckuh236/files/sarble/data_common/nibrs-user-manual-2021-1041521.pdf" ;
                rdfs:label "Animal Cruelty"@en ;
                <http://www.w3.org/2004/02/skos/core#definition> "Intentionally, knowingly, or recklessly taking an action that mistreats or kills any animal without just cause, such as torturing, tormenting, mutilation, maiming, poisoning, or abandonment. Included are instances of duty to provide care, e.g., shelter, food, water, care if sick or injured; transporting or confining an animal to fight with another; inflicting excessive or repeated unnecessary pain or suffering, e.g., uses objects to beat or injure an animal. This definition does not include proper maintenance of animals for show or sport; use of animals for food, lawful hunting, fishing or trapping." .


###  http://www.semanticweb.org/alecsculley/ontologies/crimeontology/CrO_0000008
:CrO_0000008 rdf:type owl:Class ;
       rdfs:subClassOf :CrO_0000004 ;
       rdfs:isDefinedBy "https://bjs.ojp.gov/sites/g/files/xyckuh236/files/sarble/data_common/nibrs-user-manual-2021-1041521.pdf" ;
       rdfs:label "Arson"@en ;
       <http://www.w3.org/2004/02/skos/core#definition> "To unlawfully and intentionally damage or attempt to damage any real or personal property of another person or entity by fire or incendiary device." .


###  http://www.semanticweb.org/alecsculley/ontologies/crimeontology/CrO_0000009
:CrO_0000009 rdf:type owl:Class ;
         rdfs:subClassOf :CrO_0000003 ;
         rdfs:isDefinedBy "https://bjs.ojp.gov/sites/g/files/xyckuh236/files/sarble/data_common/nibrs-user-manual-2021-1041521.pdf" ;
         rdfs:label "Assault" ;
         <http://www.w3.org/2004/02/skos/core#definition> "An unlawful attack by one person upon another." ;
         <http://www.w3.org/2004/02/skos/core#prefLabel> "Assault Offense"@en .


###  http://www.semanticweb.org/alecsculley/ontologies/crimeontology/CrO_0000010
:CrO_0000010 rdf:type owl:Class ;
         rdfs:subClassOf :CrO_0000037 ;
         rdfs:isDefinedBy "https://bjs.ojp.gov/sites/g/files/xyckuh236/files/sarble/data_common/nibrs-user-manual-2021-1041521.pdf" ;
         rdfs:label "Betting" ;
         <http://www.w3.org/2004/02/skos/core#definition> "To unlawfully stake money or something else of value on the happening of an uncertain event or on the ascertainment of a fact in dispute." ;
         <http://www.w3.org/2004/02/skos/core#prefLabel> "Betting/Wagering"@en .


###  http://www.semanticweb.org/alecsculley/ontologies/crimeontology/CrO_0000011
:CrO_0000011 rdf:type owl:Class ;
         rdfs:subClassOf :CrO_0000004 ;
         rdfs:isDefinedBy "https://bjs.ojp.gov/sites/g/files/xyckuh236/files/sarble/data_common/nibrs-user-manual-2021-1041521.pdf" ;
         rdfs:label "Bribery"@en ;
         <http://www.w3.org/2004/02/skos/core#definition> "The offering, giving, receiving, or soliciting anything of value (e.g., a bribe, gratuity, or kickback) to sway the judgement or action of a person in a position of trust or influence." .


###  http://www.semanticweb.org/alecsculley/ontologies/crimeontology/CrO_0000012
:CrO_0000012 rdf:type owl:Class ;
          rdfs:subClassOf :CrO_0000004 ;
          rdfs:isDefinedBy "https://bjs.ojp.gov/sites/g/files/xyckuh236/files/sarble/data_common/nibrs-user-manual-2021-1041521.pdf" ;
          rdfs:label "Burglary" ;
          <http://www.w3.org/2004/02/skos/core#definition> "The unlawful entry into a building or some other structure to commit a felony or a theft." ;
          <http://www.w3.org/2004/02/skos/core#prefLabel> "Burglary/Breaking & Entering"@en .


###  http://www.semanticweb.org/alecsculley/ontologies/crimeontology/CrO_0000013
:CrO_0000013 rdf:type owl:Class ;
              rdfs:subClassOf :CrO_0000034 ;
              rdfs:comment "CC fraud and ATM fraud are two different crimes" ;
              rdfs:isDefinedBy "https://bjs.ojp.gov/sites/g/files/xyckuh236/files/sarble/data_common/nibrs-user-manual-2021-1041521.pdf" ;
              rdfs:label "Credit Card/Automated Teller Machine Fraud"@en ;
              <http://www.w3.org/2004/02/skos/core#definition> "The unlawful use of a credit/debit card, credit/debit card number, or automatic teller machine for fraudulent purposes." .


###  http://www.semanticweb.org/alecsculley/ontologies/crimeontology/CrO_0000014
:CrO_0000014 rdf:type owl:Class ;
                    rdfs:subClassOf :CrO_0000005 ;
                    rdfs:label "Commerce Violation"@en .


###  http://www.semanticweb.org/alecsculley/ontologies/crimeontology/CrO_0000015
:CrO_0000015 rdf:type owl:Class ;
                        rdfs:subClassOf :CrO_0000035 ;
                        rdfs:isDefinedBy "https://bjs.ojp.gov/sites/g/files/xyckuh236/files/sarble/data_common/nibrs-user-manual-2021-1041521.pdf" ;
                        rdfs:label "Concealing from Arrest" ;
                        <http://www.w3.org/2004/02/skos/core#definition> "To harbor or conceal any person for whose arrest, a warrant or process has been issued, so as to prevent the fugitive's discovery and arrest, after having notice or knowledge that a warrant or process has been issued for the fugitive's apprehension." ;
                        <http://www.w3.org/2004/02/skos/core#prefLabel> "Harboring Escapee/Concealing from Arrest"@en .


###  http://www.semanticweb.org/alecsculley/ontologies/crimeontology/CrO_0000016
:CrO_0000016 rdf:type owl:Class ;
                rdfs:subClassOf :CrO_0000004 ;
                rdfs:isDefinedBy "https://bjs.ojp.gov/sites/g/files/xyckuh236/files/sarble/data_common/nibrs-user-manual-2021-1041521.pdf" ;
                rdfs:label "Counterfeiting" ;
                <http://www.w3.org/2004/02/skos/core#altLabel> "Forgery" ;
                <http://www.w3.org/2004/02/skos/core#definition> "The altering, copying, or imitating of something, without authority or right, with the intent to deceive or defraud by passing the copy or thing altered or imitated as that which is original or genuine, or the selling, buying, or possession of an altered, copied, or imitated thing with the intent to deceive or defraud." ;
                <http://www.w3.org/2004/02/skos/core#prefLabel> "Counterfeiting/Forgery"@en .


###  http://www.semanticweb.org/alecsculley/ontologies/crimeontology/CrO_0000001
:CrO_0000001 rdf:type owl:Class ;
       rdfs:subClassOf <http://www.ontologyrepository.com/CommonCoreOntologies/Act> ;
       <http://purl.org/dc/elements/1.1/creator> "Alec Sculley" ;
       rdfs:label "Crime"@en ;
       <http://www.w3.org/2004/02/skos/core#definition> "A crime is an act for which some law prescribes some punishment." .


###  http://www.semanticweb.org/alecsculley/ontologies/crimeontology/CrO_0000003
:CrO_0000003 rdf:type owl:Class ;
                        rdfs:subClassOf :CrO_0000001 ;
                        <http://www.ontologyrepository.com/CommonCoreOntologies/definition_source> "https://bjs.ojp.gov/sites/g/files/xyckuh236/files/sarble/data_common/nibrs-user-manual-2021-1041521.pdf" ;
                        rdfs:label "Crime Against a Person"@en ;
                        <http://www.w3.org/2004/02/skos/core#definition> "A crime against a person is a crime whose victim is some individual." .


###  http://www.semanticweb.org/alecsculley/ontologies/crimeontology/CrO_0000004
:CrO_0000004 rdf:type owl:Class ;
                        rdfs:subClassOf :CrO_0000001 ;
                        <http://www.ontologyrepository.com/CommonCoreOntologies/definition_source> "https://bjs.ojp.gov/sites/g/files/xyckuh236/files/sarble/data_common/nibrs-user-manual-2021-1041521.pdf" ;
                        rdfs:label "Crime Against Property"@en ;
                        <http://www.w3.org/2004/02/skos/core#definition> "A crime against property is a crime that has the objective to obtain money, property, or some other benefit." .


###  http://www.semanticweb.org/alecsculley/ontologies/crimeontology/CrO_0000005
:CrO_0000005 rdf:type owl:Class ;
                       rdfs:subClassOf :CrO_0000001 ;
                       <http://www.ontologyrepository.com/CommonCoreOntologies/definition_source> "https://bjs.ojp.gov/sites/g/files/xyckuh236/files/sarble/data_common/nibrs-user-manual-2021-1041521.pdf" ;
                       rdfs:label "Crime Against Society"@en ;
                       <http://www.w3.org/2004/02/skos/core#definition> "A crime against society is a crime that society prohibits, but which is not a crime against persons or a crime against property." .


###  http://www.semanticweb.org/alecsculley/ontologies/crimeontology/CrO_0000002
:CrO_0000002 rdf:type owl:Class ;
                   rdfs:subClassOf <http://purl.obolibrary.org/obo/BFO_0000015> ;
                   rdfs:label "Criminal Incident"@en .


###  http://www.semanticweb.org/alecsculley/ontologies/crimeontology/CrO_0000017
:CrO_0000017 rdf:type owl:Class ;
                          rdfs:subClassOf :CrO_0000018 ;
                          rdfs:isDefinedBy "https://bjs.ojp.gov/sites/g/files/xyckuh236/files/sarble/data_common/nibrs-user-manual-2021-1041521.pdf" ;
                          rdfs:label "Drug Equipment Violation"@en ;
                          <http://www.w3.org/2004/02/skos/core#definition> "The unlawful manufacture, sale, purchase, possession, or transportation of equipment or devices utilized in preparing and/or using drugs or narcotics." .


###  http://www.semanticweb.org/alecsculley/ontologies/crimeontology/CrO_0000018
:CrO_0000018 rdf:type owl:Class ;
              rdfs:subClassOf :CrO_0000005 ;
              rdfs:isDefinedBy "https://bjs.ojp.gov/sites/g/files/xyckuh236/files/sarble/data_common/nibrs-user-manual-2021-1041521.pdf" ;
              rdfs:label "Drug Offense" ;
              <http://www.w3.org/2004/02/skos/core#definition> "The violation of laws prohibiting the production, distribution, and/or use of certain controlled substances and the equipment or devices utilized in their preparation and/or use." ;
              <http://www.w3.org/2004/02/skos/core#prefLabel> "Drug/Narcotic Offense"@en .


###  http://www.semanticweb.org/alecsculley/ontologies/crimeontology/CrO_0000019
:CrO_0000019 rdf:type owl:Class ;
                rdfs:subClassOf :CrO_0000018 ;
                rdfs:isDefinedBy "https://bjs.ojp.gov/sites/g/files/xyckuh236/files/sarble/data_common/nibrs-user-manual-2021-1041521.pdf" ;
                rdfs:label "Drug Violation" ;
                <http://www.w3.org/2004/02/skos/core#definition> "The unlawful cultivation, manufacture, distribution, sale, purchase, use, possession, transportation, or importation of any controlled substance." ;
                <http://www.w3.org/2004/02/skos/core#prefLabel> "Drug/Narcotic Violation"@en .


###  http://www.semanticweb.org/alecsculley/ontologies/crimeontology/CrO_0000020
:CrO_0000020 rdf:type owl:Class ;
              rdfs:subClassOf :CrO_0000004 ;
              rdfs:isDefinedBy "https://bjs.ojp.gov/sites/g/files/xyckuh236/files/sarble/data_common/nibrs-user-manual-2021-1041521.pdf" ;
              rdfs:label "Embezzlement"@en ;
              <http://www.w3.org/2004/02/skos/core#definition> "The unlawful misappropriation by an offender to his/her own use or purpose of money, property, or some other thing of value entrusted to his/her care, custody, or control." .


###  http://www.semanticweb.org/alecsculley/ontologies/crimeontology/CrO_0000021
:CrO_0000021 rdf:type owl:Class ;
           rdfs:subClassOf :CrO_0000005 ;
           rdfs:isDefinedBy "https://bjs.ojp.gov/sites/g/files/xyckuh236/files/sarble/data_common/nibrs-user-manual-2021-1041521.pdf" ;
           rdfs:label "Espionage"@en ;
           <http://www.w3.org/2004/02/skos/core#definition> "The act of obtaining, delivering, transmitting, communicating, or receiving national security or national defense information with an intent, or reason to believe, that the information may be used to the injury of the United States or to the advantage of any foreign nation." .


###  http://www.semanticweb.org/alecsculley/ontologies/crimeontology/CrO_0000022
:CrO_0000022 rdf:type owl:Class ;
                     rdfs:subClassOf :CrO_0000076 ;
                     rdfs:isDefinedBy "https://bjs.ojp.gov/sites/g/files/xyckuh236/files/sarble/data_common/nibrs-user-manual-2021-1041521.pdf" ;
                     rdfs:label "Explosive Violation"@en ;
                     <http://www.w3.org/2004/02/skos/core#definition> "To knowingly violate the federal law prohibiting the manufacture, importation, sale, purchases, transfer, possession, unlawful use, intra or interstate transportation, or improper storage of any chemical compound mixture the primary or common purpose of which is to function by explosion including explosive materials or any explosive bomb, rocket, grenade, missile, or similar device, or any incendiary bomb or grenade, fire bomb, or “Molotov cocktail”." .


###  http://www.semanticweb.org/alecsculley/ontologies/crimeontology/CrO_0000023
:CrO_0000023 rdf:type owl:Class ;
                  rdfs:subClassOf :CrO_0000014 ;
                  rdfs:isDefinedBy "https://bjs.ojp.gov/sites/g/files/xyckuh236/files/sarble/data_common/nibrs-user-manual-2021-1041521.pdf" ;
                  rdfs:label "Export Violation"@en ;
                  <http://www.w3.org/2004/02/skos/core#definition> "To knowingly or willfully defraud the United States by smuggling, exporting, or clandestinely distributing merchandise that should have been invoiced, received, bought, sold, or facilitate the transportation, the concealment, or sale of such merchandise after exportation." .


###  http://www.semanticweb.org/alecsculley/ontologies/crimeontology/CrO_0000024
:CrO_0000024 rdf:type owl:Class ;
           rdfs:subClassOf :CrO_0000004 ;
           rdfs:isDefinedBy "https://bjs.ojp.gov/sites/g/files/xyckuh236/files/sarble/data_common/nibrs-user-manual-2021-1041521.pdf" ;
           rdfs:label "Extortion" ;
           <http://www.w3.org/2004/02/skos/core#altLabel> "Blackmail" ;
           <http://www.w3.org/2004/02/skos/core#definition> "To unlawfully obtain money, property, or any other thing of value, either tangible or intangible, through the use or threat of force, misuse of authority, threat of criminal prosecution, threat of destruction of reputation or social standing, or through other coercive means." ;
           <http://www.w3.org/2004/02/skos/core#prefLabel> "Extortion/Blackmail"@en .


###  http://www.semanticweb.org/alecsculley/ontologies/crimeontology/CrO_0000025
:CrO_0000025 rdf:type owl:Class ;
                       rdfs:subClassOf :CrO_0000037 ;
                       rdfs:isDefinedBy "https://bjs.ojp.gov/sites/g/files/xyckuh236/files/sarble/data_common/nibrs-user-manual-2021-1041521.pdf" ;
                       rdfs:label "Facilitating Gambling" ;
                       <http://www.w3.org/2004/02/skos/core#definition> "To unlawfully operate, promote, or assist in the operation of a game of chance, lottery, or other gambling activity." ;
                       <http://www.w3.org/2004/02/skos/core#prefLabel> "Operating/Promoting/Assisting Gambling"@en .


###  http://www.semanticweb.org/alecsculley/ontologies/crimeontology/CrO_0000026
:CrO_0000026 rdf:type owl:Class ;
                           rdfs:subClassOf :CrO_0000058 ;
                           rdfs:isDefinedBy "https://bjs.ojp.gov/sites/g/files/xyckuh236/files/sarble/data_common/nibrs-user-manual-2021-1041521.pdf" ;
                           rdfs:label "Facilitating Prostitution" ;
                           <http://www.w3.org/2004/02/skos/core#definition> "To solicit customers or transport persons for prostitution purposes; to own, manage, or operate a dwelling or other establishment for the purpose of providing a place where prostitution is performed; or to otherwise assist or promote prostitution." ;
                           <http://www.w3.org/2004/02/skos/core#prefLabel> "Assisting or Promoting Prostitution"@en .


###  http://www.semanticweb.org/alecsculley/ontologies/crimeontology/CrO_0000027
:CrO_0000027 rdf:type owl:Class ;
                                       rdfs:subClassOf :CrO_0000005 ;
                                       rdfs:comment "NIBRS 2021 says this is a sex offense, but there is no sexual act involved in this offense. So, it is not a sex offense." ;
                                       rdfs:isDefinedBy "https://bjs.ojp.gov/sites/g/files/xyckuh236/files/sarble/data_common/nibrs-user-manual-2021-1041521.pdf" ;
                                       rdfs:label "Failure to Register as a Sex Offender"@en ;
                                       <http://www.w3.org/2004/02/skos/core#definition> "To fail to register or keep current a registration as required by state and federal laws." .


###  http://www.semanticweb.org/alecsculley/ontologies/crimeontology/CrO_0000028
:CrO_0000028 rdf:type owl:Class ;
                   rdfs:subClassOf :CrO_0000045 ;
                   rdfs:isDefinedBy "https://bjs.ojp.gov/sites/g/files/xyckuh236/files/sarble/data_common/nibrs-user-manual-2021-1041521.pdf" ;
                   rdfs:label "False Citizenship"@en ;
                   <http://www.w3.org/2004/02/skos/core#definition> "Falsely and willfully representing oneself to be a citizen of the United States." .


###  http://www.semanticweb.org/alecsculley/ontologies/crimeontology/CrO_0000029
:CrO_0000029 rdf:type owl:Class ;
                        rdfs:subClassOf :CrO_0000014 ;
                        rdfs:isDefinedBy "https://bjs.ojp.gov/sites/g/files/xyckuh236/files/sarble/data_common/nibrs-user-manual-2021-1041521.pdf" ;
                        rdfs:label "Federal Liquor Offense"@en ;
                        <http://www.w3.org/2004/02/skos/core#definition> "The unlawful production (using an unregistered still), transportation (without proper bill of lading), receipt, distribution, or smuggling of distilled spirits on which federal tax has not been paid. Acting as a distiller, a winery, or a wholesaler of distilled spirits, wine, or malt beverages without a federal permit." .


###  http://www.semanticweb.org/alecsculley/ontologies/crimeontology/CrO_0000030
:CrO_0000030 rdf:type owl:Class ;
                         rdfs:subClassOf :CrO_0000014 ;
                         rdfs:isDefinedBy "https://bjs.ojp.gov/sites/g/files/xyckuh236/files/sarble/data_common/nibrs-user-manual-2021-1041521.pdf" ;
                         rdfs:label "Federal Tobacco Offense"@en ;
                         <http://www.w3.org/2004/02/skos/core#definition> "The unlawful possession and/or distribution of contraband tobacco products; including any quantity of cigarettes in excess of 10,000 or other tobacco products if the cigarettes/products bear no evidence of the payment of applicable state taxes in the state where the cigarettes are found.  Engaging in interstate commerce in tobacco products without registering with, and reporting to, the federal government and applicable state tax administrators." .


###  http://www.semanticweb.org/alecsculley/ontologies/crimeontology/CrO_0000031
:CrO_0000031 rdf:type owl:Class ;
                             rdfs:subClassOf :CrO_0000035 ;
                             rdfs:isDefinedBy "https://bjs.ojp.gov/sites/g/files/xyckuh236/files/sarble/data_common/nibrs-user-manual-2021-1041521.pdf" ;
                             rdfs:label "Flight to Avoid Deportation"@en ;
                             <http://www.w3.org/2004/02/skos/core#definition> "To knowingly leave the jurisdiction with intent to avoid deportation." .


###  http://www.semanticweb.org/alecsculley/ontologies/crimeontology/CrO_0000032
:CrO_0000032 rdf:type owl:Class ;
                             rdfs:subClassOf :CrO_0000035 ;
                             rdfs:isDefinedBy "https://bjs.ojp.gov/sites/g/files/xyckuh236/files/sarble/data_common/nibrs-user-manual-2021-1041521.pdf" ;
                             rdfs:label "Flight to Avoid Prosecution"@en ;
                             <http://www.w3.org/2004/02/skos/core#definition> "To knowingly leave the jurisdiction where charges were filed with intent to avoid prosecution, custody, confinement, or to avoid giving testimony in any criminal proceedings." .


###  http://www.semanticweb.org/alecsculley/ontologies/crimeontology/CrO_0000033
:CrO_0000033 rdf:type owl:Class ;
          rdfs:subClassOf :CrO_0000063 ;
          rdfs:isDefinedBy "https://bjs.ojp.gov/sites/g/files/xyckuh236/files/sarble/data_common/nibrs-user-manual-2021-1041521.pdf" ;
          rdfs:label "Fondling"@en ;
          <http://www.w3.org/2004/02/skos/core#definition> "The touching of the private body parts of another person for the purpose of sexual gratification, without the consent of the victim, including instances where the victim is unable to give consent because of his/her age or because of his/her temporary or permanent mental or physical incapacity." .


###  http://www.semanticweb.org/alecsculley/ontologies/crimeontology/CrO_0000034
:CrO_0000034 rdf:type owl:Class ;
       rdfs:subClassOf :CrO_0000004 ;
       rdfs:isDefinedBy "https://bjs.ojp.gov/sites/g/files/xyckuh236/files/sarble/data_common/nibrs-user-manual-2021-1041521.pdf" ;
       rdfs:label "Fraud" ;
       <http://www.w3.org/2004/02/skos/core#definition> "The intentional perversion of the truth for the purpose of inducing another person or other entity in reliance upon it to part with something of value or to surrender a legal right." ;
       <http://www.w3.org/2004/02/skos/core#prefLabel> "Fraud Offense"@en .


###  http://www.semanticweb.org/alecsculley/ontologies/crimeontology/CrO_0000035
:CrO_0000035 rdf:type owl:Class ;
                  rdfs:subClassOf :CrO_0000005 ;
                  rdfs:label "Fugitive Offense"@en .


###  http://www.semanticweb.org/alecsculley/ontologies/crimeontology/CrO_0000036
:CrO_0000036 rdf:type owl:Class ;
                              rdfs:subClassOf :CrO_0000037 ;
                              rdfs:isDefinedBy "https://bjs.ojp.gov/sites/g/files/xyckuh236/files/sarble/data_common/nibrs-user-manual-2021-1041521.pdf" ;
                              rdfs:label "Gambling Equipment Violation"@en ;
                              <http://www.w3.org/2004/02/skos/core#definition> "To unlawfully manufacture, sell, buy, possess, or transport equipment, devices, and/or goods used for gambling purposes." .


###  http://www.semanticweb.org/alecsculley/ontologies/crimeontology/CrO_0000037
:CrO_0000037 rdf:type owl:Class ;
                  rdfs:subClassOf :CrO_0000005 ;
                  rdfs:isDefinedBy "https://bjs.ojp.gov/sites/g/files/xyckuh236/files/sarble/data_common/nibrs-user-manual-2021-1041521.pdf" ;
                  rdfs:label "Gambling Offense"@en ;
                  <http://www.w3.org/2004/02/skos/core#definition> "To unlawfully bet or wager money or something else of value; assist, promote, or operate a game of chance for money or some other stake; possess or transmit wagering information; manufacture, sell, purchase, possess, or transport gambling equipment, devices, or goods; or tamper with the outcome of a sporting event or contest to gain a gambling advantage." .


###  http://www.semanticweb.org/alecsculley/ontologies/crimeontology/CrO_0000038
:CrO_0000038 rdf:type owl:Class ;
         rdfs:subClassOf :CrO_0000034 ;
         rdfs:isDefinedBy "https://bjs.ojp.gov/sites/g/files/xyckuh236/files/sarble/data_common/nibrs-user-manual-2021-1041521.pdf" ;
         rdfs:label "Hacking" ;
         <http://www.w3.org/2004/02/skos/core#definition> "Gaining access to another person’s or institution’s computer software, hardware, or networks without authorized permissions." ;
         <http://www.w3.org/2004/02/skos/core#prefLabel> "Hacking/Computer Invasion"@en .


###  http://www.semanticweb.org/alecsculley/ontologies/crimeontology/CrO_0000039
:CrO_0000039 rdf:type owl:Class ;
          rdfs:subClassOf :CrO_0000003 ;
          rdfs:isDefinedBy "https://bjs.ojp.gov/sites/g/files/xyckuh236/files/sarble/data_common/nibrs-user-manual-2021-1041521.pdf" ;
          rdfs:label "Homicide" ;
          <http://www.w3.org/2004/02/skos/core#definition> "The killing of one human being by another." ;
          <http://www.w3.org/2004/02/skos/core#prefLabel> "Homicide Offense"@en .


###  http://www.semanticweb.org/alecsculley/ontologies/crimeontology/CrO_0000040
:CrO_0000040 rdf:type owl:Class ;
                   rdfs:subClassOf :CrO_0000003 ;
                   rdfs:isDefinedBy "https://bjs.ojp.gov/sites/g/files/xyckuh236/files/sarble/data_common/nibrs-user-manual-2021-1041521.pdf" ;
                   rdfs:label "Human Trafficking"@en ;
                   <http://www.w3.org/2004/02/skos/core#definition> "The inducement of a person to perform a commercial sex act, or labor, or services, through force, fraud, or coercion.  Human trafficking has also occurred if a person under 18 years of age has been induced, or enticed, regardless of force, fraud, or coercion, to perform a commercial sex act." .


###  http://www.semanticweb.org/alecsculley/ontologies/crimeontology/CrO_0000041
:CrO_0000041 rdf:type owl:Class ;
                                      rdfs:subClassOf :CrO_0000040 ;
                                      owl:disjointWith :human_trafficking_involuntary_servitude ;
                                      rdfs:isDefinedBy "https://bjs.ojp.gov/sites/g/files/xyckuh236/files/sarble/data_common/nibrs-user-manual-2021-1041521.pdf" ;
                                      rdfs:label "Human Trafficking, Commercial Sex Act"@en ;
                                      <http://www.w3.org/2004/02/skos/core#definition> "Inducing a person by force, fraud, or coercion to participate in commercial sex acts, or in which the person induced to perform such act(s) has not attained 18 years of age." .


###  http://www.semanticweb.org/alecsculley/ontologies/crimeontology/CrO_0000042
:CrO_0000042 rdf:type owl:Class ;
                                         rdfs:subClassOf :CrO_0000040 ;
                                         rdfs:isDefinedBy "https://bjs.ojp.gov/sites/g/files/xyckuh236/files/sarble/data_common/nibrs-user-manual-2021-1041521.pdf" ;
                                         rdfs:label "Human Trafficking, Involuntary Servitude"@en ;
                                         <http://www.w3.org/2004/02/skos/core#definition> "The obtaining of person(s) through recruitment, harboring, transportation, or provision, and subjecting such persons by force, fraud, or coercion into involuntary servitude, peonage, debt bondage, or slavery (not to include commercial sex acts)." .


###  http://www.semanticweb.org/alecsculley/ontologies/crimeontology/CrO_0000043
:CrO_0000043 rdf:type owl:Class ;
                rdfs:subClassOf :CrO_0000034 ;
                rdfs:isDefinedBy "https://bjs.ojp.gov/sites/g/files/xyckuh236/files/sarble/data_common/nibrs-user-manual-2021-1041521.pdf" ;
                rdfs:label "Identity Theft"@en ;
                <http://www.w3.org/2004/02/skos/core#definition> "Wrongfully obtaining and/or using another person’s personal data (e.g., name and date of birth, Social Security number, driver’s license number)." .


###  http://www.semanticweb.org/alecsculley/ontologies/crimeontology/CrO_0000044
:CrO_0000044 rdf:type owl:Class ;
                                      rdfs:subClassOf :CrO_0000045 ;
                                      rdfs:isDefinedBy "https://bjs.ojp.gov/sites/g/files/xyckuh236/files/sarble/data_common/nibrs-user-manual-2021-1041521.pdf" ;
                                      rdfs:label "Illegal Entry into the United States"@en ;
                                      <http://www.w3.org/2004/02/skos/core#definition> "To attempt to enter the U.S. at any time or place other than as designated; or eludes examination/inspection by immigration officers." .


###  http://www.semanticweb.org/alecsculley/ontologies/crimeontology/CrO_0000045
:CrO_0000045 rdf:type owl:Class ;
                       rdfs:subClassOf :CrO_0000005 ;
                       rdfs:label "Immigration Violation"@en .


###  http://www.semanticweb.org/alecsculley/ontologies/crimeontology/CrO_0000046
:CrO_0000046 rdf:type owl:Class ;
               rdfs:subClassOf :CrO_0000034 ;
               rdfs:isDefinedBy "https://bjs.ojp.gov/sites/g/files/xyckuh236/files/sarble/data_common/nibrs-user-manual-2021-1041521.pdf" ;
               rdfs:label "Impersonation"@en ;
               <http://www.w3.org/2004/02/skos/core#definition> "Unlawfully representing one’s position and acting in the character or position to deceive others and thereby gain a profit or advantage, or enjoy some right or privilege." .


###  http://www.semanticweb.org/alecsculley/ontologies/crimeontology/CrO_0000047
:CrO_0000047 rdf:type owl:Class ;
                  rdfs:subClassOf :CrO_0000014 ;
                  rdfs:isDefinedBy "https://bjs.ojp.gov/sites/g/files/xyckuh236/files/sarble/data_common/nibrs-user-manual-2021-1041521.pdf" ;
                  rdfs:label "Import Violation"@en ;
                  <http://www.w3.org/2004/02/skos/core#definition> "To knowingly or willfully defraud the United States by smuggling, importing, or clandestinely introducing merchandise that should have been invoiced, received, bought, sold, or facilitate the transportation, the concealment, or sale of such merchandise after importation." .


###  http://www.semanticweb.org/alecsculley/ontologies/crimeontology/CrO_0000048
:CrO_0000048 rdf:type owl:Class ;
        rdfs:subClassOf :CrO_0000063 ;
        rdfs:isDefinedBy "https://bjs.ojp.gov/sites/g/files/xyckuh236/files/sarble/data_common/nibrs-user-manual-2021-1041521.pdf" ;
        rdfs:label "Incest"@en ;
        <http://www.w3.org/2004/02/skos/core#definition> "Nonforcible sexual intercourse between persons who are related to each other within the degrees wherein marriage is prohibited by law." .


###  http://www.semanticweb.org/alecsculley/ontologies/crimeontology/CrO_0000049
:CrO_0000049 rdf:type owl:Class ;
              rdfs:subClassOf :CrO_0000009 ;
              rdfs:isDefinedBy "https://bjs.ojp.gov/sites/g/files/xyckuh236/files/sarble/data_common/nibrs-user-manual-2021-1041521.pdf" ;
              rdfs:label "Intimidation"@en ;
              <http://www.w3.org/2004/02/skos/core#definition> "To unlawfully place another person in reasonable fear of harm through the use of threatening words and/or other conduct without displaying a dangerous weapon or subjecting the victim to an actual physical attack." .


###  http://www.semanticweb.org/alecsculley/ontologies/crimeontology/CrO_0000050
:CrO_0000050 rdf:type owl:Class ;
            rdfs:subClassOf :CrO_0000003 ;
            rdfs:isDefinedBy "https://bjs.ojp.gov/sites/g/files/xyckuh236/files/sarble/data_common/nibrs-user-manual-2021-1041521.pdf" ;
            rdfs:label "Kidnapping" ;
            <http://www.w3.org/2004/02/skos/core#definition> "The unlawful seizure, transportation, and/or detention of a person against his/her will or of a minor without the consent of his/her custodial parent(s) or legal guardian." ;
            <http://www.w3.org/2004/02/skos/core#prefLabel> "Kidnapping/Abduction"@en .


###  http://www.semanticweb.org/alecsculley/ontologies/crimeontology/CrO_0000051
:CrO_0000051 rdf:type owl:Class ;
                  rdfs:subClassOf :CrO_0000005 ;
                  rdfs:isDefinedBy "https://bjs.ojp.gov/sites/g/files/xyckuh236/files/sarble/data_common/nibrs-user-manual-2021-1041521.pdf" ;
                  rdfs:label "Money Laundering"@en ;
                  <http://www.w3.org/2004/02/skos/core#definition> "The process of transforming the profits of a crime into a legitimate asset." .


###  http://www.semanticweb.org/alecsculley/ontologies/crimeontology/CrO_0000052
:CrO_0000052 rdf:type owl:Class ;
                     rdfs:subClassOf :CrO_0000071 ;
                     rdfs:isDefinedBy "https://bjs.ojp.gov/sites/g/files/xyckuh236/files/sarble/data_common/nibrs-user-manual-2021-1041521.pdf" ;
                     rdfs:label "Motor Vehicle Theft"@en ;
                     <http://www.w3.org/2004/02/skos/core#definition> "The theft of a motor vehicle." .


###  http://www.semanticweb.org/alecsculley/ontologies/crimeontology/CrO_0000053
:CrO_0000053 rdf:type owl:Class ;
                                      rdfs:subClassOf :CrO_0000039 ;
                                      owl:disjointWith :negligent_manslaughter ;
                                      rdfs:isDefinedBy "https://bjs.ojp.gov/sites/g/files/xyckuh236/files/sarble/data_common/nibrs-user-manual-2021-1041521.pdf" ;
                                      rdfs:label "Murder and Nonnegligent Manslaughter"@en ;
                                      <http://www.w3.org/2004/02/skos/core#definition> "The willful (nonnegligent) killing of one human being by another." .


###  http://www.semanticweb.org/alecsculley/ontologies/crimeontology/CrO_0000054
:CrO_0000054 rdf:type owl:Class ;
                        rdfs:subClassOf :CrO_0000039 ;
                        rdfs:isDefinedBy "https://bjs.ojp.gov/sites/g/files/xyckuh236/files/sarble/data_common/nibrs-user-manual-2021-1041521.pdf" ;
                        rdfs:label "Negligent Manslaughter"@en ;
                        <http://www.w3.org/2004/02/skos/core#definition> "The killing of another person through gross negligence." .


###  http://www.semanticweb.org/alecsculley/ontologies/crimeontology/CrO_0000055
:CrO_0000055 rdf:type owl:Class ;
                            rdfs:subClassOf :CrO_0000005 ;
                            rdfs:isDefinedBy "https://bjs.ojp.gov/sites/g/files/xyckuh236/files/sarble/data_common/nibrs-user-manual-2021-1041521.pdf" ;
                            rdfs:label "Obscene Material Violation" ;
                            <http://www.w3.org/2004/02/skos/core#definition> "The violation of laws or ordinances prohibiting the manufacture, publishing (publication), distributing (distribution), sale, purchase, or possession of sexually explicit material deemed legally obscene." ;
                            <http://www.w3.org/2004/02/skos/core#prefLabel> "Pornography/Obscene Material"@en .


###  http://www.semanticweb.org/alecsculley/ontologies/crimeontology/CrO_0000056
:CrO_0000056 rdf:type owl:Class ;
             rdfs:subClassOf :CrO_0000034 ;
             rdfs:isDefinedBy "https://bjs.ojp.gov/sites/g/files/xyckuh236/files/sarble/data_common/nibrs-user-manual-2021-1041521.pdf" ;
             rdfs:label "Other Fraud" ;
             <http://www.w3.org/2004/02/skos/core#definition> "The intentional misrepresentation of existing fact or condition or the use of some other deceptive scheme or device to obtain money, goods, or other things of value. Only includes fraud offenses that do not fit any of the definitions of the specific subcategories of fraud." ;
             <http://www.w3.org/2004/02/skos/core#prefLabel> "False Pretenses/Swindle/Confidence Game"@en .


###  http://www.semanticweb.org/alecsculley/ontologies/crimeontology/CrO_0000057
:CrO_0000057 rdf:type owl:Class ;
              rdfs:subClassOf :CrO_0000058 ;
              rdfs:isDefinedBy "https://bjs.ojp.gov/sites/g/files/xyckuh236/files/sarble/data_common/nibrs-user-manual-2021-1041521.pdf" ;
              rdfs:label "Prostitution"@en ;
              <http://www.w3.org/2004/02/skos/core#definition> "To engage in commercial sex acts for anything of value." .


###  http://www.semanticweb.org/alecsculley/ontologies/crimeontology/CrO_0000058
:CrO_0000058 rdf:type owl:Class ;
                      rdfs:subClassOf :CrO_0000005 ;
                      rdfs:isDefinedBy "https://bjs.ojp.gov/sites/g/files/xyckuh236/files/sarble/data_common/nibrs-user-manual-2021-1041521.pdf" ;
                      rdfs:label "Prostitution Offense"@en ;
                      <http://www.w3.org/2004/02/skos/core#definition> "To unlawfully engage in or promote sexual activities for anything of value." .


###  http://www.semanticweb.org/alecsculley/ontologies/crimeontology/CrO_0000059
:CrO_0000059 rdf:type owl:Class ;
                         rdfs:subClassOf :CrO_0000058 ;
                         rdfs:isDefinedBy "https://bjs.ojp.gov/sites/g/files/xyckuh236/files/sarble/data_common/nibrs-user-manual-2021-1041521.pdf" ;
                         rdfs:label "Purchasing Prostitution"@en ;
                         <http://www.w3.org/2004/02/skos/core#definition> "To purchase or trade anything of value for sex acts." .


###  http://www.semanticweb.org/alecsculley/ontologies/crimeontology/CrO_0000060
:CrO_0000060 rdf:type owl:Class ;
      rdfs:subClassOf :CrO_0000063 ;
      rdfs:isDefinedBy "https://bjs.ojp.gov/sites/g/files/xyckuh236/files/sarble/data_common/nibrs-user-manual-2021-1041521.pdf" ;
      rdfs:label "Rape"@en ;
      <http://www.w3.org/2004/02/skos/core#definition> "The carnal knowledge of a person, without the consent of the victim, including instances where the victim is unable to give consent because of his/her age or because of his/her temporary or permanent mental or physical incapacity." .


###  http://www.semanticweb.org/alecsculley/ontologies/crimeontology/CrO_0000061
:CrO_0000061 rdf:type owl:Class ;
                           rdfs:subClassOf :CrO_0000045 ;
                           rdfs:isDefinedBy "https://bjs.ojp.gov/sites/g/files/xyckuh236/files/sarble/data_common/nibrs-user-manual-2021-1041521.pdf" ;
                           rdfs:label "Re-entry After Deportation"@en ;
                           <http://www.w3.org/2004/02/skos/core#definition> "The act of entering, attempting to enter, or being found in the United States after being removed, excluded, deported, or has departed the United States while an order of removal exclusion or deportation is outstanding." .


###  http://www.semanticweb.org/alecsculley/ontologies/crimeontology/CrO_0000062
:CrO_0000062 rdf:type owl:Class ;
         rdfs:subClassOf :CrO_0000004 ;
         rdfs:isDefinedBy "https://bjs.ojp.gov/sites/g/files/xyckuh236/files/sarble/data_common/nibrs-user-manual-2021-1041521.pdf" ;
         rdfs:label "Robbery"@en ;
         <http://www.w3.org/2004/02/skos/core#definition> "The taking of anything of value from the control, custody, or care of another person by force or threat of force and/or by putting the victim in fear of immediate harm." .


###  http://www.semanticweb.org/alecsculley/ontologies/crimeontology/CrO_0000063
:CrO_0000063 rdf:type owl:Class ;
             rdfs:subClassOf :CrO_0000003 ;
             rdfs:isDefinedBy "https://bjs.ojp.gov/sites/g/files/xyckuh236/files/sarble/data_common/nibrs-user-manual-2021-1041521.pdf" ;
             rdfs:label "Sex Offense"@en ;
             <http://www.w3.org/2004/02/skos/core#definition> """#1: Any sexual act directed against another person, without the consent of the victim, including instances where the victim is incapable of giving consent.

#2: Unlawful sexual intercourse.""" .


###  http://www.semanticweb.org/alecsculley/ontologies/crimeontology/CrO_0000064
:CrO_0000064 rdf:type owl:Class ;
                               rdfs:subClassOf :CrO_0000063 ;
                               rdfs:isDefinedBy "https://bjs.ojp.gov/sites/g/files/xyckuh236/files/sarble/data_common/nibrs-user-manual-2021-1041521.pdf" ;
                               rdfs:label "Sexual Assault with an Object"@en ;
                               <http://www.w3.org/2004/02/skos/core#definition> "To use an object or instrument to unlawfully penetrate, however slightly, the genital or anal opening of the body of another person, without the consent of the victim, including instances where the victim is unable to give consent because of his/her age or because of his/her temporary or permanent mental or physical incapacity." .


###  http://www.semanticweb.org/alecsculley/ontologies/crimeontology/CrO_0000065
:CrO_0000065 rdf:type owl:Class ;
                rdfs:subClassOf :CrO_0000009 ;
                rdfs:isDefinedBy "https://bjs.ojp.gov/sites/g/files/xyckuh236/files/sarble/data_common/nibrs-user-manual-2021-1041521.pdf" ;
                rdfs:label "Simple Assault"@en ;
                <http://www.w3.org/2004/02/skos/core#definition> "An unlawful physical attack by one person upon another where neither the offender displays a dangerous weapon, nor the victim suffers obvious severe or aggravated bodily injury involving apparent broken bones, loss of teeth, possible internal injury, severe laceration, or loss of consciousness." .


###  http://www.semanticweb.org/alecsculley/ontologies/crimeontology/CrO_0000066
:CrO_0000066 rdf:type owl:Class ;
                  rdfs:subClassOf :CrO_0000045 ;
                  rdfs:isDefinedBy "https://bjs.ojp.gov/sites/g/files/xyckuh236/files/sarble/data_common/nibrs-user-manual-2021-1041521.pdf" ;
                  rdfs:label "Smuggling Aliens"@en ;
                  <http://www.w3.org/2004/02/skos/core#definition> "To knowingly assist, abet, or aid another person to enter, or try to enter, the United States illegally." .


###  http://www.semanticweb.org/alecsculley/ontologies/crimeontology/CrO_0000067
:CrO_0000067 rdf:type owl:Class ;
        rdfs:subClassOf :CrO_0000063 ;
        rdfs:isDefinedBy "https://bjs.ojp.gov/sites/g/files/xyckuh236/files/sarble/data_common/nibrs-user-manual-2021-1041521.pdf" ;
        rdfs:label "Sodomy"@en ;
        <http://www.w3.org/2004/02/skos/core#definition> "Oral or anal sexual intercourse with another person, without the consent of the victim, including instances where the victim is unable to give consent because of his/her age or because of his/her temporary or permanent mental or physical incapacity." .


###  http://www.semanticweb.org/alecsculley/ontologies/crimeontology/CrO_0000068
:CrO_0000068 rdf:type owl:Class ;
                  rdfs:subClassOf :CrO_0000037 ;
                  rdfs:isDefinedBy "https://bjs.ojp.gov/sites/g/files/xyckuh236/files/sarble/data_common/nibrs-user-manual-2021-1041521.pdf" ;
                  rdfs:label "Sports Tampering"@en ;
                  <http://www.w3.org/2004/02/skos/core#definition> "To unlawfully alter, meddle in, or otherwise interfere with a sporting contest or event for the purpose of gaining a gambling advantage." .


###  http://www.semanticweb.org/alecsculley/ontologies/crimeontology/CrO_0000069
:CrO_0000069 rdf:type owl:Class ;
                rdfs:subClassOf :CrO_0000063 ;
                rdfs:isDefinedBy "https://bjs.ojp.gov/sites/g/files/xyckuh236/files/sarble/data_common/nibrs-user-manual-2021-1041521.pdf" ;
                rdfs:label "Statutory Rape"@en ;
                <http://www.w3.org/2004/02/skos/core#definition> "Nonforcible sexual intercourse with a person who is under the statutory age of consent." .


###  http://www.semanticweb.org/alecsculley/ontologies/crimeontology/CrO_0000070
:CrO_0000070 rdf:type owl:Class ;
                         rdfs:subClassOf :CrO_0000004 ;
                         rdfs:isDefinedBy "https://bjs.ojp.gov/sites/g/files/xyckuh236/files/sarble/data_common/nibrs-user-manual-2021-1041521.pdf" ;
                         rdfs:label "Stolen Property Offense"@en ;
                         <http://www.w3.org/2004/02/skos/core#definition> "Buying, receiving, possessing, selling, concealing, or transporting any property with the knowledge that it has been unlawfully taken, as by burglary, embezzlement, fraud, larceny, robbery, etc." .


###  http://www.semanticweb.org/alecsculley/ontologies/crimeontology/CrO_0000071
:CrO_0000071 rdf:type owl:Class ;
       rdfs:subClassOf :CrO_0000004 ;
       rdfs:isDefinedBy "https://bjs.ojp.gov/sites/g/files/xyckuh236/files/sarble/data_common/nibrs-user-manual-2021-1041521.pdf" ;
       rdfs:label "Theft" ;
       <http://www.w3.org/2004/02/skos/core#altLabel> "Larceny" ;
       <http://www.w3.org/2004/02/skos/core#definition> "The unlawful taking, carrying, leading, or riding away of property from the possession or constructive possession of another person." ;
       <http://www.w3.org/2004/02/skos/core#prefLabel> "Larceny/Theft Offense"@en .


###  http://www.semanticweb.org/alecsculley/ontologies/crimeontology/CrO_0000072
:CrO_0000072 rdf:type owl:Class ;
         rdfs:subClassOf :CrO_0000005 ;
         rdfs:isDefinedBy "https://bjs.ojp.gov/sites/g/files/xyckuh236/files/sarble/data_common/nibrs-user-manual-2021-1041521.pdf" ;
         rdfs:label "Treason"@en ;
         <http://www.w3.org/2004/02/skos/core#definition> "Whoever, owing allegiance to the United States, levies war against them or adheres to their enemies, giving them aid and comfort within the United States or elsewhere." .


###  http://www.semanticweb.org/alecsculley/ontologies/crimeontology/CrO_0000073
:CrO_0000073 rdf:type owl:Class ;
           rdfs:subClassOf :CrO_0000004 ;
           rdfs:isDefinedBy "https://bjs.ojp.gov/sites/g/files/xyckuh236/files/sarble/data_common/nibrs-user-manual-2021-1041521.pdf" ;
           rdfs:label "Vandalism" ;
           <http://www.w3.org/2004/02/skos/core#definition> "To willfully or maliciously destroy, damage, deface, or otherwise injure any public or private property without the consent of the owner or the person having custody or control of it." ;
           <http://www.w3.org/2004/02/skos/core#prefLabel> "Destruction/Damage/Vandalism of Property"@en .


###  http://www.semanticweb.org/alecsculley/ontologies/crimeontology/CrO_0000074
:CrO_0000074 rdf:type owl:Class ;
                                           rdfs:subClassOf :CrO_0000076 ;
                                           rdfs:isDefinedBy "https://bjs.ojp.gov/sites/g/files/xyckuh236/files/sarble/data_common/nibrs-user-manual-2021-1041521.pdf" ;
                                           rdfs:label "Violation of National Firearms Act of 1934"@en ;
                                           <http://www.w3.org/2004/02/skos/core#definition> "To manufacture, import, sell, purchase, transfer, possess, or transport in interstate commerce, a firearm knowing it has the characteristics or features of a short barreled rifle or shotgun, machine gun, silencer, destructive device, or any other weapon as defined at 26 USC § 5845(a) in violation of the provisions of the National Firearms Act (generally non-tax paid, unregistered)." .


###  http://www.semanticweb.org/alecsculley/ontologies/crimeontology/CrO_0000075
:CrO_0000075 rdf:type owl:Class ;
                                      rdfs:subClassOf :CrO_0000076 ;
                                      rdfs:isDefinedBy "https://bjs.ojp.gov/sites/g/files/xyckuh236/files/sarble/data_common/nibrs-user-manual-2021-1041521.pdf" ;
                                      rdfs:label "Weapon of Mass Destruction Violation"@en ;
                                      <http://www.w3.org/2004/02/skos/core#definition> "To knowingly violate the federal law prohibiting the unlawful use, attempted use, conspiracy to use, or use of interstate travel or facilities in furtherance of the use of a weapon of mass destruction as defined by federal law." .


###  http://www.semanticweb.org/alecsculley/ontologies/crimeontology/CrO_0000076
:CrO_0000076 rdf:type owl:Class ;
                  rdfs:subClassOf :CrO_0000005 ;
                  rdfs:isDefinedBy "https://bjs.ojp.gov/sites/g/files/xyckuh236/files/sarble/data_common/nibrs-user-manual-2021-1041521.pdf" ;
                  rdfs:label "Weapon Violation" ;
                  <http://www.w3.org/2004/02/skos/core#definition> "The violation of laws or ordinances prohibiting the manufacture, sale, purchase, transportation, possession, concealment, or use of firearms, cutting instruments, explosives, incendiary devices, or other deadly weapons." ;
                  <http://www.w3.org/2004/02/skos/core#prefLabel> "Weapon Law Violation"@en .


###  http://www.semanticweb.org/alecsculley/ontologies/crimeontology/CrO_0000077
:CrO_0000077 rdf:type owl:Class ;
               rdfs:subClassOf :CrO_0000034 ;
               rdfs:isDefinedBy "https://bjs.ojp.gov/sites/g/files/xyckuh236/files/sarble/data_common/nibrs-user-manual-2021-1041521.pdf" ;
               rdfs:label "Welfare Fraud"@en ;
               <http://www.w3.org/2004/02/skos/core#definition> "The use of deceitful statements, practices, or devices to unlawfully obtain welfare benefits." .


###  http://www.semanticweb.org/alecsculley/ontologies/crimeontology/CrO_0000078
:CrO_0000078 rdf:type owl:Class ;
                      rdfs:subClassOf :CrO_0000014 ;
                      rdfs:isDefinedBy "https://bjs.ojp.gov/sites/g/files/xyckuh236/files/sarble/data_common/nibrs-user-manual-2021-1041521.pdf" ;
                      rdfs:label "Wildlife Trafficking"@en ;
                      <http://www.w3.org/2004/02/skos/core#definition> "The poaching or other illegal taking of protected or managed species and the illegal trade in wildlife and their related parts and products." .


###  http://www.semanticweb.org/alecsculley/ontologies/crimeontology/CrO_0000079
:CrO_0000079 rdf:type owl:Class ;
            rdfs:subClassOf :CrO_0000034 ;
            rdfs:isDefinedBy "https://bjs.ojp.gov/sites/g/files/xyckuh236/files/sarble/data_common/nibrs-user-manual-2021-1041521.pdf" ;
            rdfs:label "Wire Fraud"@en ;
            <http://www.w3.org/2004/02/skos/core#definition> "The use of an electric or electronic communications facility to intentionally transmit a false and/or deceptive message in furtherance of a fraudulent activity." .


###  http://www.semanticweb.org/alecsculley/ontologies/crimeontology/CrO_0000080
:CrO_0000080 rdf:type owl:Class ;
                                                                                                                 rdfs:subClassOf :CrO_0000071 ;
                                                                                                                 rdfs:isDefinedBy "https://bjs.ojp.gov/sites/g/files/xyckuh236/files/sarble/data_common/nibrs-user-manual-2021-1041521.pdf" ;
                                                                                                                 rdfs:label "Pocket-picking"@en ;
                                                                                                                 <http://www.w3.org/2004/02/skos/core#definition> "The theft of articles from another person’s physical possession by stealth where the victim is not immediately aware a theft occurred." .


###  http://www.semanticweb.org/alecsculley/ontologies/crimeontology/CrO_0000081
:CrO_0000081 rdf:type owl:Class ;
                                                                                                                 rdfs:subClassOf :CrO_0000071 ;
                                                                                                                 rdfs:isDefinedBy "https://bjs.ojp.gov/sites/g/files/xyckuh236/files/sarble/data_common/nibrs-user-manual-2021-1041521.pdf" ;
                                                                                                                 rdfs:label "Theft from Motor Vehicle"@en ;
                                                                                                                 <http://www.w3.org/2004/02/skos/core#definition> "The unlawful taking of articles from a motor vehicle, locked or unlocked." .


###  http://www.semanticweb.org/alecsculley/ontologies/crimeontology/CrO_0000082
:CrO_0000082 rdf:type owl:Class ;
                                                                                                                 rdfs:subClassOf :CrO_0000071 ;
                                                                                                                 rdfs:isDefinedBy "https://bjs.ojp.gov/sites/g/files/xyckuh236/files/sarble/data_common/nibrs-user-manual-2021-1041521.pdf" ;
                                                                                                                 rdfs:label "Shoplifting"@en ;
                                                                                                                 <http://www.w3.org/2004/02/skos/core#definition> "The unlawful taking of goods or merchandise exposed for sale by a person (other than an employee)." .


###  http://www.semanticweb.org/alecsculley/ontologies/crimeontology/CrO_0000083
:CrO_0000083 rdf:type owl:Class ;
                                                                                                                 rdfs:subClassOf :CrO_0000071 ;
                                                                                                                 rdfs:isDefinedBy "https://bjs.ojp.gov/sites/g/files/xyckuh236/files/sarble/data_common/nibrs-user-manual-2021-1041521.pdf" ;
                                                                                                                 rdfs:label "Theft from Coin-Operated Machine or Device"@en ;
                                                                                                                 <http://www.w3.org/2004/02/skos/core#definition> "The unlawful taking of items from a machine or device that is operated or activated by the use of coins." .


###  http://www.semanticweb.org/alecsculley/ontologies/crimeontology/CrO_0000084
:CrO_0000084 rdf:type owl:Class ;
                                                                                                                 rdfs:subClassOf :CrO_0000071 ;
                                                                                                                 rdfs:isDefinedBy "https://bjs.ojp.gov/sites/g/files/xyckuh236/files/sarble/data_common/nibrs-user-manual-2021-1041521.pdf" ;
                                                                                                                 rdfs:label "Theft from Building"@en ;
                                                                                                                 <http://www.w3.org/2004/02/skos/core#definition> "The unlawful taking of items from within a building which is either open to the general public or to which the offender has legal access." .


###  http://www.semanticweb.org/alecsculley/ontologies/crimeontology/CrO_0000085
:CrO_0000085 rdf:type owl:Class ;
                                                                                                                 rdfs:subClassOf :CrO_0000071 ;
                                                                                                                 rdfs:isDefinedBy "https://bjs.ojp.gov/sites/g/files/xyckuh236/files/sarble/data_common/nibrs-user-manual-2021-1041521.pdf" ;
                                                                                                                 rdfs:label "Theft of Motor Vehicle Parts or Accessories"@en ;
                                                                                                                 <http://www.w3.org/2004/02/skos/core#definition> "The unlawful taking of any part or accessory affixed to the interior or exterior of a motor vehicle in a manner which would make the item an attachment of the vehicle or necessary for its operation." .


###  http://www.semanticweb.org/alecsculley/ontologies/crimeontology/CrO_0000086
:CrO_0000086 rdf:type owl:Class ;
                                                                                                                 rdfs:subClassOf :CrO_0000071 ;
                                                                                                                 rdfs:isDefinedBy "https://bjs.ojp.gov/sites/g/files/xyckuh236/files/sarble/data_common/nibrs-user-manual-2021-1041521.pdf" ;
                                                                                                                 rdfs:label "Purse-snatching"@en ;
                                                                                                                 <http://www.w3.org/2004/02/skos/core#definition> "The grabbing or snatching of a purse, handbag, etc., from the physical possession of another person." .


###  http://www.semanticweb.org/alecsculley/ontologies/crimeontology/CrO_0000087
:CrO_0000087 rdf:type owl:Class ;
                                                                                                                 rdfs:subClassOf :CrO_0000071 ;
                                                                                                                 rdfs:isDefinedBy "https://bjs.ojp.gov/sites/g/files/xyckuh236/files/sarble/data_common/nibrs-user-manual-2021-1041521.pdf" ;
                                                                                                                 rdfs:label "All Other Larceny"@en ;
                                                                                                                 <http://www.w3.org/2004/02/skos/core#definition> "All thefts which do not fit any of the Larceny/Theft or specific subcategories identified in UCR." .


#################################################################
#    General axioms
#################################################################

[ rdf:type owl:AllDisjointClasses ;
  owl:members ( <http://purl.obolibrary.org/obo/BFO_0000182>
                :CrO_0000001
                :CrO_0000002
              )
] .


[ rdf:type owl:AllDisjointClasses ;
  owl:members ( :CrO_0000006
                :CrO_0000049
                :CrO_0000065
              )
] .


[ rdf:type owl:AllDisjointClasses ;
  owl:members ( :CrO_0000007
                :CrO_0000014
                :CrO_0000017
                :CrO_0000019
                :CrO_0000021
                :CrO_0000027
                :CrO_0000035
                :CrO_0000037
                :CrO_0000045
                :CrO_0000051
                :CrO_0000055
                :CrO_0000058
                :CrO_0000072
                :CrO_0000076
              )
] .


[ rdf:type owl:AllDisjointClasses ;
  owl:members ( :CrO_0000008
                :CrO_0000011
                :CrO_0000012
                :CrO_0000016
                :CrO_0000020
                :CrO_0000024
                :CrO_0000034
                :CrO_0000052
                :CrO_0000062
                :CrO_0000070
                :CrO_0000071
                :CrO_0000073
              )
] .


[ rdf:type owl:AllDisjointClasses ;
  owl:members ( :CrO_0000009
                :CrO_0000039
                :CrO_0000040
                :CrO_0000050
                :CrO_0000063
              )
] .


[ rdf:type owl:AllDisjointClasses ;
  owl:members ( :CrO_0000010
                :CrO_0000026
                :CrO_0000036
                :CrO_0000068
              )
] .


[ rdf:type owl:AllDisjointClasses ;
  owl:members ( :CrO_0000013
                :CrO_0000038
                :CrO_0000043
                :CrO_0000046
                :CrO_0000056
                :CrO_0000077
                :CrO_0000079
              )
] .


[ rdf:type owl:AllDisjointClasses ;
  owl:members ( :CrO_0000015
                :CrO_0000031
                :CrO_0000032
              )
] .


[ rdf:type owl:AllDisjointClasses ;
  owl:members ( :CrO_0000003
                :CrO_0000004
                :CrO_0000005
              )
] .


[ rdf:type owl:AllDisjointClasses ;
  owl:members ( :CrO_0000022
                :CrO_0000074
                :CrO_0000075
              )
] .


[ rdf:type owl:AllDisjointClasses ;
  owl:members ( :CrO_0000023
                :CrO_0000029
                :CrO_0000030
                :CrO_0000047
                :CrO_0000078
              )
] .


[ rdf:type owl:AllDisjointClasses ;
  owl:members ( :CrO_0000026
                :CrO_0000057
                :CrO_0000059
              )
] .


[ rdf:type owl:AllDisjointClasses ;
  owl:members ( :CrO_0000028
                :CrO_0000044
                :CrO_0000061
                :CrO_0000066
              )
] .


[ rdf:type owl:AllDisjointClasses ;
  owl:members ( :CrO_0000033
                :CrO_0000048
                :CrO_0000060
                :CrO_0000064
                :CrO_0000067
                :CrO_0000069
              )
] .


[ rdf:type owl:AllDisjointClasses ;
  owl:members ( :CrO_0000052
                :CrO_0000087
                :CrO_0000081
                :CrO_0000082
                :CrO_0000083
                :CrO_0000084
                :CrO_0000085
                :CrO_0000086
                :CrO_0000087
              )
] .


###  Generated by the OWL API (version 4.5.9.2019-02-01T07:24:44Z) https://github.com/owlcs/owlapi
